checkpoint for eval; finish pass on vfa

eval/eval.py
@@ -1,7 +1,9 @@
 #!/usr/bin/env python3
 
 import os, sys
-import shutil; sys.path.append(os.path.dirname(os.path.realpath(__file__)))
+import shutil
+
+sys.path.append(os.path.dirname(os.path.realpath(__file__)))
 
 from dataclasses import dataclass
 from typing import ParamSpec, TypeVar, final, Generic, Any
@@ -18,7 +20,7 @@ from sexpdata import Symbol, parse
 
 import coq_serapy as serapi_instance
 
-from coq_serapy import kill_comments, possibly_starting_proof
+from coq_serapy import kill_comments
 
 # from coq_serapy_scraper.util import eprint, mybarfmt
 
@@ -28,7 +30,27 @@ import logging
 logging.basicConfig(
   format='%(asctime)s %(levelname)-8s %(message)s',
   level=logging.INFO,
+  stream=sys.stdout,
   datefmt='%Y-%m-%d %H:%M:%S')
+
+from os import chdir, getcwd
+
+_stack = []
+
+def pushd(dir):
+    global _stack
+    _stack.append(getcwd())
+    chdir(dir)
+
+def popd():
+    chdir(_stack.pop())
+
+match_redirect = r"-R ([a-zA-Z0-9_\-.]+) ([a-zA-Z0-9_\-.]+)"
+
+def replace_redirects(s: str, prefix: str):
+  def replacer(m: re.Match):
+    return f"-R {prefix + '/' + m.group(1)},{m.group(2)}"
+  return re.sub(match_redirect, replacer, s)
 
 
 def main():
@@ -37,6 +59,7 @@ def main():
   parser.add_argument('-j', '--threads', default=1, type=int)
   parser.add_argument('-c', '--continue', dest='cont', default=False, const=True, action='store_const')
   parser.add_argument('--hardfail', default=False, const=True, action='store_const')
+  parser.add_argument('--type', default=False, const=True, action='store_const')
   parser.add_argument('--prelude', default=".")
   parser.add_argument('-v', '--verbose', action='count', default=0)
   parser.add_argument("--progress", "-P", help="show progress of files", action='store_const', const=True, default=False)
@@ -45,15 +68,25 @@ def main():
                       dest='skip_nochange_tac')
   parser.add_argument('inputs', nargs="+", help="proof file name(s) (*.v)")
   args = parser.parse_args()
-
+  includes = None
   try:
-    with open(args.prelude + "/_CoqProject", 'r'):
+    with open(args.prelude + "/_CoqProject", 'r') as includesfile:
       # includes = includesfile.read()
       pass
   except FileNotFoundError:
     logging.error("Didn't find a _CoqProject file in prelude dir", args.prelude)
   # Set up the command which runs sertop.
   coqargs = ["sertop", "--implicit"]
+  # if includes:
+  #   logging.info("extra coqargs:")
+  #   logging.info(replace_redirects(includes, args.prelude))
+  #   coqargs += replace_redirects(includes, args.prelude).splitlines()
+
+  if args.type:
+    iter_file = iter_file_type
+  else:
+    iter_file = iter_file_prop
+
   if args.threads > 1:
     tasks = [(idx % args.threads, filename) for (idx, filename) in enumerate(args.inputs)]
     with multiprocessing.Pool(args.threads) as pool:
@@ -71,14 +104,17 @@ def main():
     for idx, fn in enumerate(args.inputs, start=1):
       res = iter_file(coqargs, args, (1,fn))
       match res:
-        case Inl(types):
-          logging.info(f"extracted types to: {types}")
+        case Inl(res):
+          if args.type:
+            logging.info(f"extracted types for {fn} to: {res}")
+          else:
+            logging.info(f"extracted props for {fn} to: {res}")
         case Inr(fname):
           logging.error(f"failed on file: {fname}")
 
 type_starting_patterns = [
-    r"Variable",
-    r"Definition",
+    # r"Variables?",
+    # r"Definition",
     r"Inductive",
     r"Record"]
 
@@ -109,18 +145,30 @@ class Inr(Generic[A, B], Sum[A, B]):
   x: B
 
 
-def make_fo_test (x: str):
-  return f"""\
-    MetaCoq Run ( \
-      MetaCoq.Template.TemplateMonad.Core.tmBind (MetaCoq.Template.TemplateMonad.Core.tmQuote {x}) (fun x => \
-      MetaCoq.Template.TemplateMonad.Core.tmBind (MirrorSolve.Eval.is_fo x) (fun y => \
-      MetaCoq.Template.TemplateMonad.Core.tmBind (MetaCoq.Template.TemplateMonad.Core.tmEval MetaCoq.Template.TemplateMonad.Common.all y) (fun z => \
-      MetaCoq.Template.TemplateMonad.Core.tmPrint z \
-    ))))."""
+def make_fo_type_test (x: str):
+  return f"""
+MetaCoq Run (
+  MetaCoq.Template.TemplateMonad.Core.tmBind (MetaCoq.Template.TemplateMonad.Core.tmQuoteRec {x}) (fun x => 
+  MetaCoq.Template.TemplateMonad.Core.tmBind (MirrorSolve.Eval.is_fo_type x) (fun x => 
+  MetaCoq.Template.TemplateMonad.Core.tmBind (MetaCoq.Template.TemplateMonad.Core.tmEval MetaCoq.Template.TemplateMonad.Common.all x) (fun x => 
+  MetaCoq.Template.TemplateMonad.Core.tmPrint x
+))))."""
+
+def make_fo_prop_test (x: str):
+  return f"""
+MetaCoq Run (
+  MetaCoq.Template.TemplateMonad.Core.tmBind (MirrorSolve.Eval.is_fo_const {x})  (fun x => 
+  MetaCoq.Template.TemplateMonad.Core.tmBind (MetaCoq.Template.TemplateMonad.Core.tmEval MetaCoq.Template.TemplateMonad.Common.all x) (fun x => 
+  MetaCoq.Template.TemplateMonad.Core.tmPrint x
+)))."""
 
 def add_prelude(coq: serapi_instance.SerapiInstance):
   coq.run_stmt("From MetaCoq.Template Require All Loader.")
   coq.run_stmt("Require MirrorSolve.Eval.")
+  coq.run_stmt("Local Unset Asymmetric Patterns.")
+  coq.run_stmt("Local Set Auto Template Polymorphism.")
+  coq.run_stmt("Local Obligation Tactic := Tactics.program_simpl.")
+  coq.run_stmt("Arguments eq_refl {A}%type_scope {x}, [_] _.")
 
 # [Symbol('Feedback'), 
 #   [
@@ -162,8 +210,8 @@ def parse_response(resp: Any):
   else:
     assert False
 
-def check_fo(coq: serapi_instance.SerapiInstance, x: str):
-  coq.run_stmt(make_fo_test(x))
+def check_fo(coq: serapi_instance.SerapiInstance, x: str, type_test: bool = False):
+  coq.run_stmt(make_fo_type_test(x) if type_test else make_fo_prop_test(x))
 
   _, _, the_response, _ = coq.feedbacks
 
@@ -175,7 +223,6 @@ def check_fo(coq: serapi_instance.SerapiInstance, x: str):
     logging.error(the_response)
     return Inr(None)
 
-# TODO: I don't think this works for section types at all
 def get_defn_ident(defn: re.Match[str]) -> Optional[str]:
   try:
     orig = defn[0]
@@ -189,29 +236,36 @@ def get_defn_ident(defn: re.Match[str]) -> Optional[str]:
     return None
 
 
-def iter_file(coqargs: List[str], args: argparse.Namespace, file_tuple: Tuple[int, str]) -> Sum[List[Tuple[str, Any]], str]:
+def iter_file_type(coqargs: List[str], args: argparse.Namespace, file_tuple: Tuple[int, str]) -> Sum[List[Tuple[str, Any]], str]:
   sys.setrecursionlimit(4500)
   file_idx, filename = file_tuple
-  full_filename = str(args.prelude) + "/" + filename
+  pushd(args.prelude)
+  full_filename = filename
   commands = serapi_instance.load_commands_preserve(args, file_idx, str(full_filename))
 
   try:
-    with serapi_instance.SerapiContext(
-      coqargs,
-      serapi_instance.get_module_from_filename(filename),
-      args.prelude, False) as coq:
+    with \
+      serapi_instance.SerapiContext(
+          coqargs
+        , serapi_instance.get_module_from_filename(filename)
+        , '.'
+        , False) as coq:
 
       coq.verbose = args.verbose
       ret : List[Tuple[str, Any]] = []
+      
 
       add_prelude(coq)
+
+      # coq.check_term("eq_refl 0")
+      # logging.info(coq.coq_minor_version())
 
       for cmd in commands: 
         coq.run_stmt(cmd)
         if (mtch := possibly_starting_type(cmd)):
           if (ident := get_defn_ident(mtch)):
-            
-            match check_fo(coq, ident):
+            # logging.info(f"checking type of {mtch.groups()}")
+            match check_fo(coq, ident, type_test=True):
               case Inl(r):
                 ret.append((coq.module_prefix + ident, r))
               case Inr(_):
@@ -222,6 +276,86 @@ def iter_file(coqargs: List[str], args: argparse.Namespace, file_tuple: Tuple[in
       return Inl(ret)
   except:
     return Inr(full_filename)
+  finally:
+    popd()
 
+thm_match = r".*(Theorem|Lemma|Fact|Remark|Corollary|Proposition|Property)\s+([a-zA-Z_](\w|')+)\s*(.*)" 
+
+def replace_first_semi(thm_rhs: str) -> str:
+  in_paren = 0
+  
+  for i, c in enumerate(thm_rhs):
+    if c == '(':
+      in_paren += 1
+    elif c == ')':
+      in_paren -= 1
+    elif c == ':' and not in_paren:
+      return thm_rhs[0:i] + ':=' + thm_rhs[i+1:]
+  
+  assert False
+
+def iter_file_prop(coqargs: List[str], args: argparse.Namespace, file_tuple: Tuple[int, str]) -> Sum[List[Tuple[str, Any]], str]:
+  sys.setrecursionlimit(4500)
+  file_idx, filename = file_tuple
+  pushd(args.prelude)
+  full_filename = filename
+  commands = serapi_instance.load_commands_preserve(args, file_idx, str(full_filename))
+
+  try:
+    with \
+      serapi_instance.SerapiContext(
+          coqargs
+        , serapi_instance.get_module_from_filename(filename)
+        , '.'
+        , False) as coq:
+
+      coq.verbose = args.verbose
+      ret : List[Tuple[str, Any]] = []
+
+      add_prelude(coq)
+
+      counter = 0
+
+      for cmd in commands: 
+        # logging.info(cmd)
+        if (mtch := re.match(thm_match, cmd.replace('\n', ' ').strip())):
+          # logging.info("prop to check:")
+          # logging.info(mtch.group(4))
+          name = f"ms__prop__{counter}"
+          add_cmd = f"Definition {name} {replace_first_semi(mtch.group(4))}"
+          coq.run_stmt(add_cmd)
+          # logging.info(f"added: {add_cmd}")
+
+          match check_fo(coq, name, type_test=False):
+            case Inl(r):
+              ret.append((coq.module_prefix + mtch.group(2), r))
+            case Inr(_):
+              logging.error(f"error parsing prop for {mtch.group(2)}")
+              logging.error("original command:")
+              logging.error(cmd)
+          counter += 1
+        else:
+          if serapi_instance.possibly_starting_proof(cmd):
+            # logging.warn("skipping possible proof:")
+            # logging.warn(cmd)
+            pass
+        
+
+        coq.run_stmt(cmd)
+
+      return Inl(ret)
+  except:
+    return Inr(full_filename)
+  finally:
+    popd()
+
+test = """
+Lemma nlist_forall2_imply:
+  forall (A B: Type) (P1: A -> B -> Prop) (l1: nlist A) (l2: nlist B),
+  nlist_forall2 P1 l1 l2 ->
+  forall (P2: A -> B -> Prop),
+  (forall v1 v2, nIn v1 l1 -> nIn v2 l2 -> P1 v1 v2 -> P2 v1 v2) ->
+  nlist_forall2 P2 l1 l2.
+"""
 if __name__ == "__main__":
   main()
