eval/plot.py
@@ -1,0 +1,47 @@
+#!/usr/bin/env python3
+
+import argparse
+import sys
+import re
+
+import logging
+logging.basicConfig(
+  format='%(asctime)s %(levelname)-8s %(message)s',
+  level=logging.INFO,
+  stream=sys.stdout,
+  datefmt='%Y-%m-%d %H:%M:%S')
+
+
+# convert lines of output into a list of file, typename, result
+def process_file(fp: str) -> list[str]:
+  ret : list[str] = []
+  # 2022-10-04 22:08:09 INFO     extracted types for powerpc/Builtins1.v to: [('Builtins1.platform_builtin', True)]
+  line_matcher = r".*extracted \w+ for (.+) to: \[(.*)\]"
+  # ('FIX.beta', False), ('FIX.emin', False), ('FIX.FIX_format', None)
+  with open(fp, 'r') as f:
+    for line in f:
+      if (match := re.match(line_matcher, line)):
+        # split the list of tuples into each individual tuple
+        tuples = match.group(2).split("),") if len(match.group(2)) else []
+        # split each tuple into two different items
+        tuples_split = [x.split(',') for x in tuples]
+        # clean up parens and whitespace
+        cleaned_tuples = [[x.strip().strip('(').strip(')').strip("'").replace("None", "-").replace("True", "1").replace("False","0") for x in tuple] for tuple in tuples_split]
+
+        for tup in cleaned_tuples:
+          ret.append(match.group(1) + "," + tup[0] + "," + tup[1])
+  
+  return ret
+
+def main():
+    # Parse the command line arguments.
+  parser = argparse.ArgumentParser(description="convert the output of eval into a csv")
+  parser.add_argument('-i', '--input', required=True, help="input path")
+  args = parser.parse_args()
+
+  ret = process_file(args.input)
+  for line in ret:
+    print(line)
+
+if __name__ == "__main__":
+  main()
