tests/case-studies/vfa/SearchTree.v
@@ -10,8 +10,6 @@ Require Import MirrorSolve.BV.
 Require Import MirrorSolve.SMT.
 Require Import MirrorSolve.UF.
 
-Require Import MirrorSolve.FOLTrees.
-
 Require Import MirrorSolve.HLists.
 Require Import Coq.Lists.List.
 
@@ -30,395 +28,705 @@ Require Import MirrorSolve.UF.
 Require Import MirrorSolve.Reflection.Core.
 Require Import MirrorSolve.Reflection.FM.
 Require Import MirrorSolve.Reflection.Tactics.
-(* From Hammer Require Import Hammer.
+From Hammer Require Import Hammer.
 
 Set Hammer ATPLimit 5.
-Set Hammer ReconstrLimit 10. *)
+Set Hammer ReconstrLimit 10.
 
-Local Declare ML Module "mirrorsolve".
+Require Import MirrorSolve.Crush.
 
-Create HintDb ms_db.
+Inductive sorted : list Z -> Prop :=
+  | sorted_nil : sorted []
+  | sorted_1 : forall x, sorted [x]
+  | sorted_cons : forall x y l,
+    (x <= y)%Z -> sorted (y :: l) -> sorted (x :: y :: l).
 
-Lemma foo : 1 = 1.
+Inductive NoDup_Z : list Z -> Prop :=
+  NoDup_nil_z : NoDup_Z []
+| NoDup_cons_z : forall (x : Z) (l : list Z),
+                ~ In x l -> NoDup_Z l -> NoDup_Z (x :: l).
+
+Lemma nd_z_nil : 
+  NoDup_Z [] <-> True.
 Proof.
-  exact eq_refl.
+  intuition eauto.
+  econstructor.
 Qed.
 
-Hint Immediate foo : ms_db.
+Lemma nd_z_cons : 
+  forall (x: Z) (l: list Z), 
+    NoDup_Z (x :: l) <-> (~ In x l /\ NoDup_Z l).
+Proof.
+  intros.
+  split; intros.
+  - inversion H;
+    subst.
+    intuition eauto.
+  - econstructor.
+    intuition eauto.
+    destruct H.
+    eauto.
+Qed.
 
+Definition disjoint (l1 l2: list Z) := forall (x : Z),
+  In x l1 -> ~ In x l2.
 
+Lemma disjoint_spec:
+  forall l1 l2, disjoint l1 l2 <-> (forall x, In x l1 -> ~ In x l2).
+Proof.
+  intuition eauto.
+Qed.
 
-Goal False.
-  hints_foreach (fun x => pose proof x) "ms_db".
-Abort.
-
-
-Section Trees.
-  (* type of values in the tree *)
+Section SearchTree.
   Variable (V: Type).
-  Set Universe Polymorphism.
+  Notation key := Z.
 
-  (*** MS BEGIN {"type": "configuration", "config_type":"boilerplate"} *)
-  
-  Notation sig := FOLTrees.sig.
-  
-  Definition tree_model := FOLTrees.fm_model V.
+(** [E] represents the empty map.  [T l k v r] represents the
+    map that binds [k] to [v], along with all the bindings in [l] and
+    [r].  No key may be bound more than once in the map. *)
 
-  MetaCoq Quote Definition t_ite := @ite.
-  MetaCoq Quote Definition t_zlt := @Z.ltb.
-  MetaCoq Quote Definition t_glt := @Z.gtb.
-  MetaCoq Quote Definition t_zlt' := @Z.lt.
-  MetaCoq Quote Definition t_glt' := @Z.gt.
-  MetaCoq Quote Definition t_emp := @Emp.
-  MetaCoq Quote Definition t_node := @Node.
-  MetaCoq Quote Definition t_insert := (@FOLTrees.insert V).
-  MetaCoq Quote Definition t_lookup := (@FOLTrees.lookup V).
-  MetaCoq Quote Definition t_bound := (@FOLTrees.bound V).
-  MetaCoq Quote Definition t_lt_t := (@FOLTrees.lt_t V).
-  MetaCoq Quote Definition t_gt_t := (@FOLTrees.gt_t V).
-  MetaCoq Quote Definition t_ordered := (@FOLTrees.ordered V).
-  
-  Definition is_emp t := eq_ctor t t_emp.
-  Definition is_node t := eq_ctor t t_node.
-  Definition is_zlt t := eq_term t t_zlt.
-  Definition is_zgt t := eq_term t t_glt.
-  Definition is_insert t := eq_ctor t t_insert.
-  Definition is_lookup t := eq_ctor t t_lookup.
-  Definition is_bound t := eq_ctor t t_bound.
-  Definition is_lt_t t := eq_ctor t t_lt_t.
-  Definition is_gt_t t := eq_ctor t t_gt_t.
-  Definition is_ordered t := eq_ctor t t_ordered.
-  Definition is_zlt' t := eq_term t t_zlt'.
-  Definition is_zgt' t := eq_term t t_glt'.
+  Inductive tree : Type :=
+    | E
+    | T (l : tree) (k : key) (v : V) (r : tree).
 
-  MetaCoq Quote Definition t_bool := (bool).
-  MetaCoq Quote Definition t_Z := (Z).
-  MetaCoq Quote Definition t_tree := (@tree V).
-  MetaCoq Quote Definition t_V := (V).
+  Equations empty_tree : tree := {empty_tree := E }.
 
-  Definition is_cond_b t :=
-    match t with 
-    | tApp f (t :: _) => 
-      andb (eq_term f t_ite) (eq_term t t_bool)
-    | _ => false
+  Local Open Scope Z_scope.
+
+(** [bound k t] is whether [k] is bound in [t]. *)
+  Equations bound_t (x : key) (t: tree) : bool := {
+    bound_t _ E := false ;
+    bound_t x (T l y v r) := 
+      ite (x <? y) (bound_t x l) (
+      ite (x >? y) (bound_t x r) true
+    )
+  }.
+
+(** [lookup d k t] is the value bound to [k] in [t], or is default
+    value [d] if [k] is not bound in [t]. *)
+
+  Equations lookup_t (d : V) (x : key) (t: tree) : V := {
+    lookup_t d _ E := d ;
+    lookup_t d x (T l y v r) := 
+      ite (x <? y) (lookup_t d x l) (
+      ite (x >? y) (lookup_t d x r) v
+    );
+  }.
+
+(** [insert k v t] is the map containing all the bindings of [t] along
+    with a binding of [k] to [v]. *)
+
+  Equations insert_t (x : key) (v: V) (t: tree) : tree := {
+    insert_t x v E := T E x v E ;
+    insert_t x v (T l y v' r) := 
+      ite (x <? y) (T (insert_t x v l) y v' r) (
+      ite (x >? y) (T l y v' (insert_t x v r)) (T l x v r)
+    );
+  }.
+
+
+(** So, let's formalize the BST invariant. Here's one way to do
+    so.  First, we define a helper [ForallT] to express that idea that
+    a predicate holds at every node of a tree: *)
+
+  Fixpoint ForallT (P: key -> V -> Prop) (t: tree) : Prop :=
+    match t with
+    | E => True
+    | T l k v r => P k v /\ ForallT P l /\ ForallT P r
     end.
 
-  Definition is_cond_t t :=
+  Fixpoint lt_t (k: Z) (t: tree) : Prop := 
     match t with 
-    | tApp f (t :: _) => 
-      andb (eq_term f t_ite) (eq_term t t_V)
-    | _ => false
+    | E => True
+    | T l k' _ r => k' < k /\ lt_t k l /\ lt_t k r
+    end. 
+  
+  Lemma lt_t_spec : forall x t, ForallT (fun y _ => y < x) t <-> lt_t x t.
+  Proof.
+    induction t; simpl in *; intuition eauto.
+  Qed.
+
+  Fixpoint lt_list (k: Z) (t: list (key * V)) : Prop := 
+    match t with 
+    | [] => True
+    | (k', _) :: t' => k' < k /\ lt_list k t'
+    end. 
+
+  Fixpoint lt_list_s (k: key) (t: list key) : Prop := 
+    match t with 
+    | [] => True
+    | k' :: t' => k' < k /\ lt_list_s k t'
+    end. 
+
+  Fixpoint gt_t (k: Z) (t: tree) : Prop := 
+    match t with 
+    | E => True
+    | T l k' _ r => k' > k /\ gt_t k l /\ gt_t k r
+    end. 
+  
+  Lemma gt_t_spec : forall x t, ForallT (fun y _ => y > x) t <-> gt_t x t.
+  Proof.
+    induction t; simpl in *; intuition eauto.
+  Qed.
+
+  Fixpoint gt_list (k: Z) (t: list (key * V)) : Prop := 
+    match t with 
+    | [] => True
+    | (k', _) :: t' => k' > k /\ gt_list k t'
+    end. 
+  Fixpoint gt_list_s (k: Z) (t: list key) : Prop := 
+    match t with 
+    | [] => True
+    | k' :: t' => k' > k /\ gt_list_s k t'
+    end. 
+
+  (** Second, we define the BST invariant:
+
+      - An empty tree is a BST.
+
+      - A non-empty tree is a BST if all its left nodes have a lesser
+        key, its right nodes have a greater key, and the left and
+        right subtrees are themselves BSTs. *)
+
+  Inductive BST : tree -> Prop :=
+  | BST_E : BST E
+  | BST_T : forall l x v r,
+      ForallT (fun y _ => y < x) l ->
+      ForallT (fun y _ => y > x) r ->
+      BST l ->
+      BST r ->
+      BST (T l x v r).
+
+  (* Hint Constructors BST. *)
+  Fixpoint ordered (t: tree) : Prop :=
+    match t with 
+    | E => True
+    | T l k _ r => 
+      lt_t k l /\ 
+      gt_t k r /\ 
+      ordered l /\ ordered r
     end.
 
-  Definition is_cond_tree t :=
-    match t with 
-    | tApp f (t :: _) => 
-      andb (eq_term f t_ite) (eq_term t t_tree)
-    | _ => false
-    end.
+  Lemma ordered_spec : 
+    forall t, BST t <-> ordered t.
+  Proof.
+    induction t; simpl in *; intuition eauto;
+    try (now econstructor);
+    try match goal with 
+    | H: BST (_ _ _ _ _) |- _ => inversion H; subst
+    end;
+    intuition eauto.
+    - eapply lt_t_spec; eauto.
+    - eapply gt_t_spec; eauto.
+    - econstructor; eauto;
+      (eapply lt_t_spec || eapply gt_t_spec); eauto.
+  Qed.
 
-  Notation tac_bool_tree := (tacLit sig tree_model bool_lit (fun b => (BS; b)) (fun b _ => (BS; TFun sig (b_lit b) hnil)) ltac:(solve_lit_wf)).
-  Notation tac_fun_tree f := (tac_fun sig f).
-  Notation tac_rel_tree f := (tac_rel sig f).
 
-  Definition match_tacs : list ((term -> bool) * tac_syn sig tree_model) := [
-      ( is_emp, tac_fun_tree e_f)
-    ; ( is_node, tac_fun_tree t_f)
-    ; ( is_zlt, tac_fun_tree z_lt)
-    ; ( is_zgt, tac_fun_tree z_gt)
-    ; ( is_cond_b, tac_fun_tree cond_b)
-    ; ( is_cond_t, tac_fun_tree cond_t)
-    ; ( is_cond_tree, tac_fun_tree cond_tree)
-    ; ( is_bool_term, tac_bool_tree )
-    ; ( is_lookup, tac_fun_tree lookup_f)
-    ; ( is_bound, tac_fun_tree bound_f)
-    ; ( is_insert, tac_fun_tree insert_f)
-    ; ( is_lt_t, tac_rel_tree lt_t_r)
-    ; ( is_gt_t, tac_rel_tree gt_t_r)
-    ; ( is_ordered, tac_rel_tree ordered_r) 
-    ; ( is_zlt', tac_rel_tree lt_z)
-    ; ( is_zgt', tac_rel_tree gt_z)
+  (* This is needed for later *)
+  Equations elements (t : tree) : list (key * V) := {
+    elements E := [] ;
+    elements (T l k v r) := elements l ++ [(k, v)] ++ elements r;
+  }.
+
+  Equations map_fst (xs : list (key * V)) : list key := {
+    map_fst [] := [] ;
+    map_fst ((x, _) :: xs) := x :: map_fst xs;
+  }.
+
+  Equations fast_elements_tr (t: tree) (acc : list (key * V)) : list (key * V) := {
+    fast_elements_tr E acc := acc ;
+    fast_elements_tr (T l k v r) acc := fast_elements_tr l ((k, v) :: fast_elements_tr r acc);
+  }.
+
+  Equations fast_elements (t : tree) : list (key * V) := { 
+    fast_elements t := fast_elements_tr t [];
+  }.
+
+  Equations kvs_insert (k : key) (v : V) (kvs : list (key * V)) : list (key * V) := {
+    kvs_insert k v [] := [(k, v)] ;
+    kvs_insert k v ((k', v') :: kvs') := 
+      ite (k <? k') ((k, v) :: (k', v') :: kvs') (
+      ite (k >? k') ((k', v') :: kvs_insert k v kvs') (
+        (k, v) :: kvs'
+      ));
+  }.
+
+  Declare ML Module "mirrorsolve".
+
+  From MetaCoq.Template Require Import All Loader.
+  Import MCMonadNotation.
+  Require Import MirrorSolve.Config.
+  Open Scope bs.
+
+  (* MirrorSolve's automation needs this later. *)
+  Universe foo.
+  MetaCoq Quote Definition typ_term := Type@{foo}.
+
+  Notation pack x := (existT _ _ x).
+
+  Definition fun_syms : list packed := ([
+      pack bound_t
+    ; pack lookup_t
+    ; pack insert_t
+    ; pack tree
+    ; pack (key * V)
+    ; pack (list (key * V))
+    ; pack (list key)
+    ; pack (list V)
+    ; pack map_fst
+    ; pack (@List.app (key * V))
+    ; pack (@List.app key)
+    ; pack Z.ltb
+    ; pack Z.gtb
+    ; pack empty_tree
+    ; pack (@ite tree)
+    ; pack (@ite V)
+    ; pack (@ite bool)
+    ; pack (@ite (list (key * V)))
+    ; pack elements
+    ; pack fast_elements
+    ; pack fast_elements_tr
+    ; pack kvs_insert
+  ])%type.
+
+  Definition rel_syms : list packed := ([ 
+        pack BST
+      ; pack ordered
+      ; pack lt_t
+      ; pack gt_t
+      ; pack Z.lt
+      ; pack Z.gt
+      ; pack (@List.In (key * V))
+      ; pack (@List.In key)
+      ; pack lt_list
+      ; pack gt_list
+      ; pack lt_list_s
+      ; pack gt_list_s
+      ; pack sorted
+      ; pack (Z.le)
+      ; pack NoDup_Z
+      ; pack disjoint
+  ])%type.
+
+  Definition prim_syms : list (packed * String.string) := [
+      (pack Z.add, "+"%string)
+    ; (pack Z.lt, "<"%string)
+    ; (pack Z.gt, ">"%string)
+    ; (pack Z.ltb, "<"%string)
+    ; (pack Z.gtb, ">"%string)
+    ; (pack Z.le, "<="%string)
+    ; (pack (@ite bool), "ite"%string)
+    ; (pack (@ite tree), "ite"%string)
+    ; (pack (@ite V), "ite"%string)
+    ; (pack (@ite (list (key * V))), "ite"%string)
   ].
 
-  Definition match_inds : list ((term -> bool) * FOLTrees.sorts) := [
-      (eq_term t_tree, TreeS)
-    ; (eq_term t_V, TS)
-    ; (eq_term t_bool, BS)
-    ; (eq_term t_Z, ZS)
-  ].
+  MetaCoq Run (
+    xs <- add_funs typ_term fun_syms rel_syms ;;
+    xs' <- tmQuote xs ;;
+    tmMkDefinition "trans_tbl" xs'
+  ).
 
-  
-  (*** MS END {"type": "configuration", "config_type":"boilerplate"} *)
-  (*** MS BEGIN {"type": "configuration", "config_type":"plugin"} *)
-  RegisterCustomSort TS "A".
-  (*** MS END {"type": "configuration", "config_type":"plugin"} *)
+  MetaCoq Run (
+    gen_sig typ_term sorts fol_funs fol_rels 
+  ).
+  MetaCoq Run (
+    gen_interp_funs sorts interp_sorts fol_funs trans_tbl
+  ).
+  MetaCoq Run (
+    gen_interp_rels sorts interp_sorts fol_rels trans_tbl
+  ).
+  Definition fm_model := Build_model sig interp_sorts interp_funs interp_rels.
+  MetaCoq Run (
+    match Utils.find _ _ smt_fun_base_beq IntLit (Utils.flip trans_tbl.(mp_consts)) with 
+    | Some v => add_const_wf_instance sig fm_model v IntLit 
+    | None => tmReturn tt
+    end
+  ).
+  MetaCoq Run (
+    match Utils.find _ _ smt_fun_base_beq BoolLit (Utils.flip trans_tbl.(mp_consts)) with 
+    | Some v => add_const_wf_instance sig fm_model v BoolLit 
+    | None => tmReturn tt
+    end
+  ).
+  MetaCoq Run (
+    add_matches sig fm_model trans_tbl
+  ).
+  MetaCoq Run (
+    ctx <- build_printing_ctx sig sort_Prop trans_tbl prim_syms;; 
+    ctx' <- tmEval all ctx ;;
+    rhs <- tmQuote ctx' ;; 
+    tmMkDefinition "fol_theory" rhs
+  ).
 
-  (*** MS BEGIN {"type": "configuration", "config_type":"boilerplate"} *)
-  RegisterSMTInd TreeS (SICases [
-    ("node"%string, [SIRec; SISort (SInt tt); SISort (SCustom "A"); SIRec]); 
-    ("emp"%string, [])
-    ]) "A_tree".
-  (*** MS END {"type": "configuration", "config_type":"boilerplate"} *)
+  Require Import MirrorSolve.Reflection.Tactics.
 
-  (*** MS BEGIN {"type": "configuration", "config_type":"plugin"} *)
-
-  RegisterSMTSort ZS SInt.
-  RegisterSMTSort BS SBool.
-
-  RegisterSMTUF "bound" BS ZS TreeS.
-  RegisterSMTUF "lookup" TS TS ZS TreeS.
-  RegisterSMTUF "insert" TreeS ZS TS TreeS.
-  RegisterSMTUF "lt_t" BS ZS TreeS.
-  RegisterSMTUF "gt_t" BS ZS TreeS.
-  RegisterSMTUF "ordered" BS TreeS.
-
-  RegisterSMTFun FOLTrees.z_lt "<" 2.
-  RegisterSMTFun FOLTrees.z_gt ">" 2.
-  RegisterSMTFun FOLTrees.lt_z "<" 2.
-  RegisterSMTFun FOLTrees.gt_z ">" 2.
-  RegisterSMTFun FOLTrees.e_f "emp" 0.
-  RegisterSMTFun FOLTrees.t_f "node" 4.
-  RegisterSMTFun FOLTrees.bound_f "bound" 2.
-  RegisterSMTFun FOLTrees.lookup_f "lookup" 3.
-  RegisterSMTFun FOLTrees.insert_f "insert" 3.
-  RegisterSMTFun FOLTrees.lt_t_r "lt_t" 2.
-  RegisterSMTFun FOLTrees.gt_t_r "gt_t" 2.
-  RegisterSMTFun FOLTrees.ordered_r "ordered" 1.
-  RegisterSMTFun FOLTrees.cond_b "ite" 3.
-  RegisterSMTFun FOLTrees.cond_t "ite" 3.
-  RegisterSMTFun FOLTrees.cond_tree "ite" 3.
-
-  RegisterSMTBuiltin FOLTrees.b_lit BoolLit.
-  (*** MS END {"type": "configuration", "config_type":"plugin"} *)
-
-  (*** MS BEGIN {"type": "configuration", "config_type":"boilerplate"} *)
   Transparent denote_tm.
   Require Import MirrorSolve.Axioms.
 
+  (* We make use of the verification trick of negating the goal and checking for unsat. 
+    The check_unsat_neg tactic behaves like idtac if the negated goal is unsat and otherwise fails.
+    *)
   Ltac check_goal_unsat := 
     match goal with 
-    | |- ?G => check_unsat_neg G; eapply UnsoundAxioms.interp_true
+    | |- ?G => check_unsat_neg_func fol_theory G; eapply UnsoundAxioms.interp_true
     end.
 
-  (*** MS END {"type": "configuration", "config_type":"boilerplate"} *)
-  (*** MS BEGIN {"type": "configuration", "config_type":"tactics"} *)
-  Ltac pose_lookup_axioms := Utils.pose_all (tt, @lookup_emp V, @lookup_node V).
-  Ltac pose_bound_axioms := Utils.pose_all (tt, @bound_emp V, @bound_node V).
-  Ltac pose_insert_axioms := Utils.pose_all (tt, @insert_emp V, @insert_node V).
-  Ltac pose_ordered_axioms := Utils.pose_all (tt, @lt_t_emp V, @lt_t_node V, @gt_t_emp V, @gt_t_node V, @ordered_emp V, @ordered_node V).
-
-  Ltac pose_tree_axioms := pose_lookup_axioms; 
-    pose_bound_axioms; 
-    pose_insert_axioms; 
-    pose_ordered_axioms.
+  Create HintDb tree_eqns.
 
   Ltac prep_proof := 
+    hints_foreach (fun x => pose proof x) "tree_eqns";
     Utils.revert_all;
-    intros V;
-    pose_tree_axioms; 
-    Utils.revert_all;
-    unfold "<->";
-    intros V.
-  (*** MS END {"type": "configuration", "config_type":"tactics"} *)
+    unfold "<->" in *.
 
-  Ltac quote_reflect_tree := quote_reflect FOLTrees.sig tree_model FOLTrees.sorts_eq_dec match_tacs match_inds.
-  Ltac quote_extract_tree := quote_extract FOLTrees.sig tree_model FOLTrees.sorts_eq_dec match_tacs match_inds.
+  Scheme Equality for sorts.
 
+  Ltac quote_reflect_tree := quote_reflect sig fm_model sorts_eq_dec match_tacs match_sorts.
 
-  Ltac mirrorsolve T := 
-    T;
+  Ltac mirrorsolve :=
+    prep_proof;
     quote_reflect_tree;
-    check_goal_unsat.
+    check_goal_unsat. 
 
-  (* hammer handles this one (it's easy) *)
-  (*** MS BEGIN {"type": "configuration", "config_type":"plugin"} *)
-  SetSMTSolver "cvc5".
-  (*** MS END {"type": "configuration", "config_type":"plugin"} *)
-  (*** MS BEGIN {"type": "proof_definition"} *)
-  Theorem lookup_empty : 
-    forall (d: V) (k : Z),
-      lookup d k Emp = d.
-  (*** MS END {"type": "proof_definition"} *)
-  Proof.
-    (*** MS BEGIN {"type": "proof", "proof_type":"manual"} *)
-    intros.
-    trivial.
-    (*** MS END {"type": "proof", "proof_type":"manual"} *)
-    Restart.
-  Proof.
-    (*** MS BEGIN {"type": "proof", "proof_type":"hammer", "total":1, "finished":1} *)
-    (* hammer. *)
-    (*** MS END {"type": "proof", "proof_type":"hammer", "total":1, "finished":1} *)
-  Restart.
-  Proof.
-    (*** MS BEGIN {"type": "proof", "proof_type":"mirrorsolve", "total":1} *)
-    mirrorsolve prep_proof.
-    (*** MS END {"type": "proof", "proof_type":"mirrorsolve", "total":1} *)
-  Admitted. (* Crashes? *)
+  SetSMTSolver "z3".
 
-  (*** MS BEGIN {"type": "proof_definition"} *)
-  Theorem lookup_insert_eq : 
-    forall (t : tree V) d k k' v,
-      k = k' ->
-      lookup d k (insert k' v t)  = v.
-  (*** MS END {"type": "proof_definition"} *)
-  Proof.
-    (*** MS BEGIN {"type": "proof", "proof_type":"manual"} *)
-    induction t;
-    intros;
-    simpl in *;
-    subst.
-    - destruct (_ <? _)%Z eqn:?;
-      simpl in *; [
-          Lia.lia
-        |
-      ].
-      destruct (_ >? _)%Z eqn:?;
-      simpl in *; [
-          Lia.lia
-        | trivial
-      ].
-    - destruct (_ <? _)%Z eqn:?;
-      simpl in *.
-      * erewrite Heqb;
-        simpl;
-        eapply IHt1;
-        trivial.
-      * destruct (_ >? _)%Z eqn:?;
-        try erewrite Heqb0;
-        simpl in *;
-        try erewrite Heqb;
-        simpl;
-        try erewrite Heqb0;
-        simpl.
-        + eapply IHt2.
-          trivial.
-        + destruct (k' <? k')%Z eqn:?;
-          simpl; [
-              Lia.lia
-            |
-          ].
-          destruct (k' >? k')%Z eqn:?;
-          simpl; [
-              Lia.lia
-            | trivial
-          ]. 
-    (*** MS END {"type": "proof", "proof_type":"manual"} *)
-  Restart.
-  Proof.
-    (*** MS BEGIN {"type": "proof", "proof_type":"hammer", "total":2, "finished":0} *)
-    induction t.
-    (* - try hammer; admit.   
-    - try hammer; admit. *)
-    (*** MS END {"type": "proof", "proof_type":"hammer", "total":2, "finished":0} *)
-    Restart.
-  Proof.
-    (*** MS BEGIN {"type": "proof", "proof_type":"mirrorsolve", "total":2} *)
-    induction t;
-    mirrorsolve prep_proof.
-    (*** MS END {"type": "proof", "proof_type":"mirrorsolve", "total":2} *)
-  Admitted.
+  Hint Immediate ordered_spec : tree_eqns. 
 
-  (* hammer does not handle this one *)
-  (*** MS BEGIN {"type": "proof_definition"} *)
-  Theorem lookup_insert_neq :
-    forall (t: tree V) d k k' v,
-      k <> k' -> 
-      lookup d k' (insert k v t) = lookup d k' t.
-  (*** MS END {"type": "proof_definition"} *)
+  (*** MS BEGIN {"type": "configuration", "config_type":"boilerplate"} *)
+  Lemma ordered_emp: 
+    ordered E.
+  Proof. 
+    intros; 
+    simpl; 
+    intuition. 
+  Qed.
+
+  Lemma ordered_node: 
+    forall l k v r, 
+      (lt_t k l /\ 
+      gt_t k r /\ 
+      ordered l /\ ordered r) <->
+      ordered (T l k v r).
+  Proof. 
+    intros; 
+    simpl; 
+    intuition. 
+  Qed.
+
+  Hint Immediate ordered_emp : tree_eqns. 
+  Hint Immediate ordered_node : tree_eqns. 
+  (*** MS END {"type": "configuration", "config_type":"boilerplate"} *)
+    
+
+(** **** Exercise: 1 star, standard (empty_tree_BST) *)
+
+(** Prove that the empty tree is a BST. *)
+
+  Theorem empty_tree_BST : 
+      BST E.
   Proof.
-    (*** MS BEGIN {"type": "proof", "proof_type":"manual"} *)
+    mirrorsolve.
+  Qed.
+
+(** [] *)
+
+(** **** Exercise: 4 stars, standard (insert_BST) *)
+
+(** Prove that [insert] produces a BST, assuming it is given one.
+
+    Start by proving this helper lemma, which says that [insert]
+    preserves any node predicate. Proceed by induction on [t]. *)
+
+  (* We can't prove the helper predicate because it's about the higher-order thing of ForallT *)
+
+Lemma ForallT_insert : forall (P : key -> V -> Prop) (t : tree),
+    ForallT P t -> forall (k : key) (v : V),
+      P k v -> ForallT P (insert_t k v t).
+Proof.
+  (* FILL IN HERE *) Admitted.
+
+(* But we can prove the corresponding properties for lt_t and gt_t.
+*)
+
+  (* first, reflect lt_t and gt_t: *)
+
+  (*** MS BEGIN {"type": "configuration", "config_type":"boilerplate"} *)
+  Lemma lt_emp: 
+    forall x, lt_t x E <-> True.
+  Proof. 
+    intros; 
+    simpl; 
+    intuition. 
+  Qed.
+
+  Lemma lt_node: 
+    forall x l k v r, 
+      (lt_t x l /\ 
+       lt_t x r /\
+       k < x) <->
+      lt_t x (T l k v r).
+  Proof. 
+    intros; 
+    simpl; 
+    intuition. 
+  Qed.
+
+  Hint Immediate lt_emp : tree_eqns. 
+  Hint Immediate lt_node : tree_eqns. 
+
+  Lemma gt_emp: 
+    forall x, gt_t x E <-> True.
+  Proof. 
+    intros; 
+    simpl; 
+    intuition. 
+  Qed.
+
+  Lemma gt_node: 
+    forall x l k v r, 
+      (gt_t x l /\ 
+       gt_t x r /\
+       k > x) <->
+      gt_t x (T l k v r).
+  Proof. 
+    intros; 
+    simpl; 
+    intuition. 
+  Qed.
+
+  Hint Immediate gt_emp : tree_eqns. 
+  Hint Immediate gt_node : tree_eqns. 
+
+
+  Hint Immediate gt_emp : tree_eqns. 
+  Hint Immediate gt_node : tree_eqns. 
+
+  Hint Immediate insert_t_equation_1 : tree_eqns.
+  Hint Immediate insert_t_equation_2 : tree_eqns.
+  (*** MS END {"type": "configuration", "config_type":"boilerplate"} *)
+
+
+  Lemma gt_t_trans : 
+    forall (x y : Z), 
+      x > y -> 
+      forall t, gt_t x t -> gt_t y t.
+  Proof.
+    (* induction t;
+    try hammer.
+    Restart.  *)
+    (* hammer and crush both worked! *)
     induction t;
-    simpl in *;
-    intros.
-    - destruct (_ <? _)%Z eqn:?;
-      simpl in *; [
-          trivial
-        |
-      ].
-      destruct (_ >? _)%Z eqn:?;
-      simpl in *; [
-          trivial
-        | Lia.lia
-      ].
-    - destruct (_ <? _)%Z eqn:?;
-      simpl in *.
-      * erewrite IHt1;
-        trivial.
-      * destruct (_ >? _)%Z eqn:?;
-        simpl.
-        + erewrite IHt2;
-          trivial.
-        + assert (k0 = k) by Lia.lia.
-          subst.
-          destruct (k' <? k)%Z eqn:?; 
-          simpl in *; [
-              trivial
-            | 
-          ].
-          destruct (k' >? k)%Z eqn:?; 
-          simpl in *; [
-              trivial
-            | Lia.lia
-          ].
-    (*** MS END {"type": "proof", "proof_type":"manual"} *)
-    Restart.
+    mirrorsolve.
+  Qed.
+
+  Lemma lt_t_trans : 
+    forall (x y : Z), 
+      x < y -> 
+      forall t, lt_t x t -> lt_t y t.
   Proof.
-    (*** MS BEGIN {"type": "proof", "proof_type":"hammer", "total":2, "finished":0} *)
-    induction t. 
-    (* - try hammer. admit.
-    - try hammer. admit. *)
-    (*** MS END {"type": "proof", "proof_type":"hammer", "total":2, "finished":0} *)
-    Restart.
+    induction t;
+    mirrorsolve.
+  Qed.
+
+  Hint Immediate lt_t_trans : tree_eqns.
+  Hint Immediate gt_t_trans : tree_eqns.
+
+  Hint Immediate Z.ltb_lt : tree_eqns.
+  
+  Lemma gtb_gt : 
+    forall (x y: Z), (x >? y = true) <-> x > y.
   Proof.
-    (*** MS BEGIN {"type": "proof", "proof_type":"mirrorsolve", "total":2} *)
+    Lia.lia.
+  Qed.
+  Hint Immediate gtb_gt : tree_eqns.
+
+  Lemma lt_t_insert : 
+    forall t x k, 
+      lt_t x t->
+      k < x -> 
+      forall v, 
+        lt_t x (insert_t k v t).
+  Proof.
+    induction t;
+    mirrorsolve.
+  Qed.
+
+  Hint Immediate lt_t_insert : tree_eqns.
+
+  Lemma gt_t_insert : 
+    forall t x k, 
+      gt_t x t->
+      k > x -> 
+      forall v, 
+        gt_t x (insert_t k v t).
+  Proof.
+    induction t;
+    mirrorsolve.
+  Qed.
+  Hint Immediate gt_t_insert : tree_eqns.
+
+  Lemma ordered_insert : 
+    forall t x k, 
+      ordered t -> ordered (insert_t k x t).
+  Proof.
+    (* induction t;
+    try hammer.
+    Restart.
+    induction t;
+    try crush.
+    Restart. *)
+    (* hammer and crush did not work here *)
+    induction t;
+    mirrorsolve.
+  Qed.
+  Hint Immediate ordered_insert : tree_eqns.
+
+
+(** Now prove the main theorem. Proceed by induction on the evidence
+    that [t] is a BST. *)
+
+  Theorem insert_BST : forall (k : key) (v : V) (t : tree),
+      BST t -> BST (insert_t k v t).
+  Proof.
+    induction t;
+    mirrorsolve.
+  Qed.
+  Hint Immediate insert_BST : tree_eqns.
+
+(** [] *)
+
+(** Since [empty_tree] and [insert] are the only operations that
+    create BSTs, we are guaranteed that any [tree] is a BST -- unless
+    it was constructed manually with [T].  It would therefore make
+    sense to limit the use of [T] to only within the tree operations,
+    rather than expose it.  Coq, like OCaml and other functional
+    languages, can do this with its module system.  See [ADT] for
+    details. *)
+
+(* ################################################################# *)
+(** * Correctness of BST Operations *)
+
+(** To prove the correctness of [lookup] and [bound], we need
+    specifications for them.  We'll study two different techniques for
+    that in this chapter. *)
+
+(** The first is called _algebraic specification_.  With it, we write
+    down equations relating the results of operations.  For example,
+    we could write down equations like the following to specify the
+    [+] and [*] operations:
+
+      (a + b) + c = a + (b + c)
+      a + b = b + a
+      a + 0 = a
+      (a * b) * c = a * (b * c)
+      a * b = b * a
+      a * 1 = a
+      a * 0 = 0
+      a * (b + c) = a * b + a * c
+
+    For BSTs, let's examine how [lookup] should interact with
+    when applied to other operations.  It is easy to see what needs to
+    be true for [empty_tree]: looking up any value at all in the empty
+    tree should fail and return the default value:
+
+      lookup d k empty_tree = d
+
+    What about non-empty trees?  The only way to build a non-empty
+    tree is by applying [insert k v t] to an existing tree [t]. So it
+    suffices to describe the behavior of [lookup] on the result of an
+    arbitrary [insert] operation. There are two cases.  If we look up
+    the same key that was just inserted, we should get the value that
+    was inserted with it:
+
+      lookup d k (insert k v t) = v
+
+    If we look up a different key than was just inserted, the insert
+    should not affect the answer -- which should be the same as if we
+    did the lookup in the original tree before the insert occured:
+
+      lookup d k' (insert k v t) = lookup d k' t      if k <> k'
+
+    These three basic equations specify the correct behavior of maps.
+    Let's prove that they hold. *)
+
+  
+  Hint Immediate empty_tree_equation_1 : tree_eqns.
+  Hint Immediate lookup_t_equation_1 : tree_eqns.
+  Hint Immediate lookup_t_equation_2 : tree_eqns.
+
+  Theorem lookup_empty : forall (d : V) (k : key),
+      lookup_t d k empty_tree = d.
+  Proof.
+    mirrorsolve.
+  Qed.
+
+  Theorem lookup_insert_eq : forall (t : tree) (d : V) (k : key) (v : V),
+      lookup_t d k (insert_t k v t)  = v.
+  Proof.
     induction t; 
-    mirrorsolve prep_proof.
-    (*** MS END {"type": "proof", "proof_type":"mirrorsolve", "total":2} *)
-  Admitted.
+    mirrorsolve.
+  Qed.
+
+  Hint Immediate lookup_insert_eq : tree_eqns.
+  Hint Immediate lookup_empty : tree_eqns.
+
+
+(** The basic method of that proof is to repeatedly [bdestruct]
+    everything in sight, followed by generous use of [lia] and
+    [auto]. Let's automate that. *)
+
+
+(** The tactic immediately pays off in proving the third
+    equation. *)
+
+  Theorem lookup_insert_neq :
+    forall (t : tree) (d : V) (k k' : key) (v : V),
+    k <> k' -> lookup_t d k' (insert_t k v t) = lookup_t d k' t.
+  Proof.
+    induction t;
+    mirrorsolve.
+  Qed.
+
+  Hint Immediate lookup_insert_neq : tree_eqns.
+
+(** Perhaps surprisingly, the proofs of these results do not
+    depend on whether [t] satisfies the BST invariant.  That's because
+    [lookup] and [insert] follow the same path through the tree, so
+    even if nodes are in the "wrong" place, they are consistently
+    "wrong". *)
+
+(** **** Exercise: 3 stars, standard, optional (bound_correct) *)
+
+(** Specify and prove the correctness of [bound]. State and prove
+    three theorems, inspired by those we just proved for [lookup]. If
+    you have the right theorem statements, the proofs should all be
+    quite easy -- thanks to [bdall]. *)
+
+(* FILL IN HERE *)
+
+(* Do not modify the following line: *)
+Definition manual_grade_for_bound_correct : option (nat*string) := None.
+(** [] *)
 
 (** **** Exercise: 3 stars, standard, optional (bound_default) *)
 
 (** Prove that if [bound] returns [false], then [lookup] returns
     the default value. Proceed by induction on the tree. *)
 
-  (*** MS BEGIN {"type": "proof_definition"} *)
+  Hint Immediate bound_t_equation_1 : tree_eqns.
+  Hint Immediate bound_t_equation_2 : tree_eqns.
+
   Theorem bound_default :
-    forall k d (t: tree V),
-      bound k t = false ->
-      lookup d k t = d.
-  (*** MS END {"type": "proof_definition"} *)
+    forall (t: tree) (k : key) (d : V),
+      bound_t k t = false ->
+      lookup_t d k t = d.
   Proof.
-    (*** MS BEGIN {"type": "proof", "proof_type":"manual"} *)
     induction t;
-    simpl in *;
-    intros; 
-    trivial.
-    destruct (_ <? _)%Z eqn:?;
-    simpl in *; [
-        intuition eauto
-      |
-    ].
-    destruct (_ >? _)%Z eqn:?;
-    simpl in *; [
-        intuition eauto
-      | congruence
-    ].
-    (*** MS END {"type": "proof", "proof_type":"manual"} *)
-    Restart.
-  Proof.
-    (*** MS BEGIN {"type": "proof", "proof_type":"hammer", "total":2, "finished":1} *)
-    induction t.
-    (* - try hammer.
-    - admit.  *)
-    (*** MS END {"type": "proof", "proof_type":"hammer", "total":2, "finished":1} *)
-    Restart.
-  Proof.
-    (*** MS BEGIN {"type": "proof", "proof_type":"mirrorsolve", "total":2} *)
-    induction t; 
-    mirrorsolve prep_proof.
-    (*** MS END {"type": "proof", "proof_type":"mirrorsolve", "total":2} *)
-  Admitted.
+    mirrorsolve.
+  Qed.
+
+  Hint Immediate bound_default : tree_eqns.
 
 (** [] *)
 
@@ -437,274 +745,43 @@ Section Trees.
 
 (** **** Exercise: 2 stars, standard, optional (lookup_insert_shadow) *)
 
-  (* hammer does not handle this one *)
-  (*** MS BEGIN {"type": "proof_definition"} *)
   Lemma lookup_insert_shadow :
-    forall (t: tree V) v v' d k k',
-      lookup d k' (insert k v (insert k v' t)) = lookup d k' (insert k v t).
-  (*** MS END {"type": "proof_definition"} *)
+    forall (t : tree) (v v' d: V) (k k' : key),
+      lookup_t d k' (insert_t k v (insert_t k v' t)) = lookup_t d k' (insert_t k v t).
   Proof.
-    (*** MS BEGIN {"type": "proof", "proof_type":"manual"} *)
     induction t;
-    simpl in *;
-    intros.
-    - assert ((k <? k)%Z = false) by Lia.lia. 
-      erewrite H;
-      simpl.
-      assert ((k >? k)%Z = false) by Lia.lia. 
-      erewrite H0;
-      simpl.
-      trivial.
-    - destruct (_ <? _)%Z eqn:?;
-      simpl in *.
-      + erewrite Heqb;
-        simpl.
-        f_equal.
-        eapply IHt1.
-      + destruct (_ >? _)%Z eqn:?;
-        simpl in *.
-        * erewrite Heqb.
-          erewrite Heqb0.
-          simpl.
-          f_equal.
-          f_equal.
-          eapply IHt2.
-        * assert ((k0 <? k0)%Z = false) by Lia.lia.
-          assert ((k0 >? k0)%Z = false) by Lia.lia.
-          erewrite H.
-          erewrite H0.
-          simpl.
-          f_equal.
-    (*** MS END {"type": "proof", "proof_type":"manual"} *)
-    Restart.   
-  Proof.
-    (*** MS BEGIN {"type": "proof", "proof_type":"hammer", "total":2, "finished":0} *)
-    induction t.
-    - admit. (* try hammer; admit.*)
-    - admit. (* try hammer; admit. *)
-    (*** MS END {"type": "proof", "proof_type":"hammer", "total":2, "finished":0} *)
-    Restart.
-  Proof.
-(*** MS BEGIN {"type": "proof", "proof_type":"mirrorsolve", "total":2} *)
-    induction t; 
-    mirrorsolve prep_proof.
-(*** MS END {"type": "proof", "proof_type":"mirrorsolve", "total":2} *)
-  Admitted.
+    mirrorsolve.
+  Qed.
 
-  (** **** Exercise: 2 stars, standard, optional (lookup_insert_same) *)
+(** [] *)
 
-  (* hammer does not handle this one *)
-  (*** MS BEGIN {"type": "proof_definition"} *)
+(** **** Exercise: 2 stars, standard, optional (lookup_insert_same) *)
+
   Lemma lookup_insert_same :
-    forall k k' d (t: tree V),
-      lookup d k' (insert k (lookup d k t) t) = lookup d k' t.
-  (*** MS END {"type": "proof_definition"} *)
+    forall (t : tree) (k k' : key) (d : V),
+      lookup_t d k' (insert_t k (lookup_t d k t) t) = lookup_t d k' t.
   Proof.
-    (*** MS BEGIN {"type": "proof", "proof_type":"manual"} *)
     induction t; 
-    simpl in *;
-    intros.
-    - destruct (_ <? _)%Z eqn:?;
-      simpl in *;
-      trivial.
-      destruct (_ >? _)%Z eqn:?;
-      simpl in *;
-      trivial.
-    - destruct (_ <? _)%Z eqn:?;
-      simpl in *;
-      trivial.
-      + f_equal.
-        eauto.
-      + destruct (_ >? _)%Z eqn:?;
-        simpl in *;
-        trivial;
-        destruct (_ <? _)%Z eqn:?;
-        simpl.
-        * f_equal.
-          f_equal.
-          eauto.
-        * f_equal;
-          f_equal;
-          eauto.
-        * congruence.
-        * f_equal; [
-            Lia.lia
-            | f_equal
-          ].
-          Lia.lia.
-    (*** MS END {"type": "proof", "proof_type":"manual"} *)
-    Restart.
-  Proof.
-    (*** MS BEGIN {"type": "proof", "proof_type":"hammer", "total":2, "finished":0} *)
-    induction t.
-    - admit.
-    - admit.
-    (*** MS END {"type": "proof", "proof_type":"hammer", "total":2, "finished":0} *)
-    Restart.
-  Proof. 
-    (*** MS BEGIN {"type": "proof", "proof_type":"mirrorsolve", "total":2} *)
-    induction t; 
-    mirrorsolve prep_proof.
-    (*** MS END {"type": "proof", "proof_type":"mirrorsolve", "total":2} *)
-  Admitted.
+    mirrorsolve.
+  Qed.
 
-  (** **** Exercise: 2 stars, standard, optional (lookup_insert_permute) *)
+  Hint Immediate lookup_insert_same : tree_eqns.
+(** [] *)
 
-  (* hammer does not handle this one *)
-  (*** MS BEGIN {"type": "proof_definition"} *)
+(** **** Exercise: 2 stars, standard, optional (lookup_insert_permute) *)
+
   Lemma lookup_insert_permute :
-    forall v1 v2 d k1 k2 k' (t: tree V),
+    forall (t: tree) (v1 v2 d : V) (k1 k2 k': key),
       k1 <> k2 ->
-      lookup d k' (insert k1 v1 (insert k2 v2 t))
-      = lookup d k' (insert k2 v2 (insert k1 v1 t)).
-  (*** MS END {"type": "proof_definition"} *)
-  Proof. 
-    (*** MS BEGIN {"type": "proof", "proof_type":"manual"} *)
-    induction t;
-    simpl in *;
-    intros.
-    - destruct (_ <? _)%Z eqn:?;  
-      simpl.
-      * assert ((k2 <? k1)%Z = false) by Lia.lia.
-        assert ((k2 >? k1)%Z = true) by Lia.lia.
-        erewrite H0.
-        erewrite H1.
-        simpl.
-        destruct (k' <? k2)%Z eqn:?;
-        simpl; [
-          trivial
-          | 
-        ].
-        destruct (k' <? k1)%Z eqn:?;
-        assert ((k' >? k1)%Z = true) by Lia.lia;
-        erewrite H2;
-        simpl.
-        + destruct (k' >? k2)%Z eqn:?;
-          simpl; [
-              trivial
-            | Lia.lia
-          ].
-        + destruct (k' >? k2)%Z eqn:?;
-          simpl;
-          trivial.
-      * assert ((k2 <? k1)%Z = true) by Lia.lia.
-        assert ((k2 >? k1)%Z = false) by Lia.lia.
-        erewrite H0.
-        erewrite H1.
-        simpl.
-        destruct (k' <? k1)%Z eqn:?;
-        simpl; 
-        assert ((k1 >? k2)%Z = true) by Lia.lia;
-        erewrite H2;
-        simpl.
-        + f_equal.
-          f_equal.
-          erewrite Heqb0;
-          trivial.
-        + destruct (k' <? k2)%Z eqn:?;
-          try Lia.lia;
-          assert ((k' >? k2)%Z = true) by Lia.lia;
-          erewrite H3;
-          erewrite Heqb0;
-          simpl;
-          f_equal.
-    - destruct (k2 <? k)%Z eqn:?;
-      destruct (k2 >? k)%Z eqn:?;
-      destruct (k1 <? k)%Z eqn:?;
-      destruct (k1 >? k)%Z eqn:?;
-      simpl;
-      try Lia.lia.
-      * erewrite Heqb1.
-        erewrite Heqb.
-        simpl.
-        f_equal;  
-        eauto.
-      * erewrite Heqb1.
-        erewrite Heqb0.
-        erewrite Heqb2.
-        erewrite Heqb.
-        simpl.
-        f_equal.
-      * erewrite Heqb1.
-        erewrite Heqb2.
-        simpl.
-        destruct (k2 <? k1)%Z eqn:?;
-        simpl;
-        trivial.
-        assert ((k2 >? k1)%Z = true) by Lia.lia.
-        erewrite H0.
-        simpl.
-        f_equal.
-        + eapply lookup_insert_neq;
-          Lia.lia.
-        + f_equal.
-          erewrite lookup_insert_neq;
-          trivial.
-          Lia.lia.
-      * erewrite Heqb1;
-        erewrite Heqb;
-        erewrite Heqb0;
-        erewrite Heqb2;
-        simpl.
-        f_equal.
-      * erewrite Heqb1;
-        erewrite Heqb;
-        erewrite Heqb0;
-        erewrite Heqb2;
-        simpl.
-        f_equal.
-        f_equal.
-        eapply IHt2.
-        trivial.
-      * erewrite Heqb1;
-        erewrite Heqb2;
-        simpl;
-        destruct (k2 <? k1)%Z eqn:?;
-        simpl;
-        try Lia.lia.
-        assert ((k2 >? k1)%Z = true) by Lia.lia.
-        erewrite H0.
-        simpl.
-        f_equal.
-      * erewrite Heqb;
-        erewrite Heqb0;
-        simpl.
-        destruct (k1 <? k2)%Z eqn:?;
-        simpl; [
-            f_equal
-          |
-        ].
-        assert ((k1 >? k2)%Z = true) by Lia.lia.
-        erewrite H0.
-        simpl.
-        f_equal;
-        try Lia.lia.
-      * erewrite Heqb;
-        erewrite Heqb0;
-        simpl.
-        destruct (k1 <? k2)%Z eqn:?;
-        simpl; [
-            Lia.lia
-          |
-        ].
-        assert ((k1 >? k2)%Z = true) by Lia.lia.
-        erewrite H0.
-        simpl.
-        f_equal.
-    (*** MS END {"type": "proof", "proof_type":"manual"} *)
-    Restart.
+      lookup_t d k' (insert_t k1 v1 (insert_t k2 v2 t))
+      = lookup_t d k' (insert_t k2 v2 (insert_t k1 v1 t)).
   Proof.
-    (*** MS BEGIN {"type": "proof", "proof_type":"hammer", "total":2, "finished":0} *)
-    induction t.
-    - admit. (* hammer. *)
-    - admit. (* hammer. *)
-    (*** MS END {"type": "proof", "proof_type":"hammer", "total":2, "finished":0} *)
-  Restart.
-  (*** MS BEGIN {"type": "proof", "proof_type":"mirrorsolve", "total":2} *)
     induction t; 
-    mirrorsolve prep_proof.
-  (*** MS END {"type": "proof", "proof_type":"mirrorsolve", "total":2} *)
-  Admitted.
+    mirrorsolve.
+  Qed.
+
+  Hint Immediate lookup_insert_permute : tree_eqns.
+(** [] *)
 
 (** Our ability to prove these lemmas without reference to the
     underlying tree implementation demonstrates they hold for any map
@@ -718,58 +795,13 @@ Section Trees.
     Could we state the tree lemmas with direct equalities?  For
     [insert_shadow], the answer is yes: *)
 
-  (* hammer does not handle this one *)
-  (*** MS BEGIN {"type": "proof_definition"} *)
-  Lemma insert_shadow_equality : 
-    forall (t: tree V) k v v',
-      insert k v (insert k v' t) = insert k v t.
-  (*** MS END {"type": "proof_definition"} *)
+  Lemma insert_shadow_equality : forall (t : tree) (k : key) (v v' : V),
+      insert_t k v (insert_t k v' t) = insert_t k v t.
   Proof.
-    (*** MS BEGIN {"type": "proof", "proof_type":"manual"} *)
-    induction t;
-    simpl in *;
-    intros.
-    - assert ((k <? k)%Z = false) by Lia.lia;
-      assert ((k >? k)%Z = false) by Lia.lia;
-      erewrite H;
-      erewrite H0;
-      simpl.
-      trivial.
-    - destruct (_ <? _)%Z eqn:?;
-      simpl.
-      * erewrite Heqb.
-        simpl.
-        f_equal.
-        eapply IHt1.
-      * destruct (k0 >? k)%Z eqn:?;
-        simpl.
-        + erewrite Heqb.
-          erewrite Heqb0.
-          simpl.
-          f_equal.
-          eapply IHt2.
-        + assert ((k0 <? k0)%Z = false) by Lia.lia.
-          erewrite H;
-          simpl.
-          assert ((k0 >? k0)%Z = false) by Lia.lia;
-          erewrite H0;
-          simpl.
-          trivial.
-    (*** MS END {"type": "proof", "proof_type":"manual"} *)
-    Restart.
-  Proof.
-    (*** MS BEGIN {"type": "proof", "proof_type":"hammer", "total":2, "finished":0} *)
-    induction t.
-    - admit. (* hammer. *)
-    - admit. (* hammer. *)
-    (*** MS END {"type": "proof", "proof_type":"hammer", "total":2, "finished":0} *)
-    Restart.
-  Proof.
-    (*** MS BEGIN {"type": "proof", "proof_type":"mirrorsolve", "total":2} *)
-    induction t; 
-    mirrorsolve prep_proof.
-    (*** MS END {"type": "proof", "proof_type":"mirrorsolve", "total":2} *)
-  Admitted.
+    induction t; mirrorsolve.
+  Qed.
+
+  Hint Immediate insert_shadow_equality : tree_eqns.
 
 (** But the other two direct equalities on BSTs do not necessarily
     hold. *)
@@ -781,242 +813,1307 @@ Section Trees.
     on your counterexample.  The simpler your counterexample, the simpler
     the rest of the proof will be. *)
 
-(* Lemma insert_same_equality_breaks :
-  exists (V : Type) (d : V) (t : tree V) (k : key),
-      insert k (lookup d k t) t <> t.
+    (* MIRRORSOLVE: We can't prove these because they use exists *)
+Lemma insert_same_equality_breaks :
+  exists (d : V) (t : tree) (k : key),
+      insert_t k (lookup_t d k t) t <> t.
 Proof.
   (* FILL IN HERE *) Admitted.
 
 Lemma insert_permute_equality_breaks :
-  exists (V : Type) (v1 v2 : V) (k1 k2 : key) (t : tree V),
-    k1 <> k2 /\ insert k1 v1 (insert k2 v2 t) <> insert k2 v2 (insert k1 v1 t).
+  exists (v1 v2 : V) (k1 k2 : key) (t : tree),
+    k1 <> k2 /\ insert_t k1 v1 (insert_t k2 v2 t) <> insert_t k2 v2 (insert_t k1 v1 t).
 Proof.
-  (* FILL IN HERE *) Admitted. *)
+  (* FILL IN HERE *) Admitted.
 
 (** [] *)
 
-(** some custom stuff, about balance and that insert preserves the balance of the tree **)
+(* ################################################################# *)
+(** * Converting a BST to a List *)
 
-SetSMTSolver "cvc5".
-(*** MS BEGIN {"type": "proof_definition"} *)
-Lemma insert_left_lt : 
-  forall (l: tree V) k k' v, 
-    (k < k')%Z -> 
-    lt_t k' l -> 
-    lt_t k' (insert k v l).
-(*** MS END {"type": "proof_definition"} *)
-Proof. 
-  (*** MS BEGIN {"type": "proof", "proof_type":"manual"} *)
-  induction l;
-  intros; 
-  simpl in *.
-  - intuition.
-  - destruct (k0 <? k)%Z eqn:?;
-    simpl in *; [
-        intuition 
-      | 
-    ].
-    destruct (k0 >? k)%Z eqn:?;
-    simpl in *; 
-    intuition.
-  (*** MS END {"type": "proof", "proof_type":"manual"} *)
-  Restart.
-Proof.
-  (*** MS BEGIN {"type": "proof", "proof_type":"hammer", "total":2, "finished":1} *)
-  induction l.
-  (* - hammer. *)
-  - admit. (* hammer. *)
-  (*** MS END {"type": "proof", "proof_type":"hammer", "total":2, "finished":1} *)
-  Restart.
-Proof.
-  (*** MS BEGIN {"type": "proof", "proof_type":"mirrorsolve", "total":2} *)
-  induction l;
-  mirrorsolve prep_proof.
-(*** MS END {"type": "proof", "proof_type":"mirrorsolve", "total":2} *)
-Admitted.
+(** Let's add a new operation to our BST: converting it to an
+    _association list_ that contains the key--value bindings from the
+    tree stored as pairs.  If that list is sorted by the keys, then
+    any two trees that represent the same map would be converted to
+    the same list. Here's a function that does so with an in-order
+    traversal of the tree: *)
 
-(*** MS BEGIN {"type": "proof_definition"} *)
-Lemma insert_right_lt : 
-  forall (r: tree V) k k' v, 
-    (k' < k)%Z -> 
-    gt_t k' r -> 
-    gt_t k' (insert k v r).
-(*** MS END {"type": "proof_definition"} *)
-Proof.
-  (*** MS BEGIN {"type": "proof", "proof_type":"manual"} *)
-  induction r;
-  intros; 
-  simpl in *.
-  - intuition.
-  - destruct (k0 <? k)%Z eqn:?;
-    simpl in *; [
-        intuition 
-      | 
-    ].
-    destruct (k0 >? k)%Z eqn:?;
-    simpl in *; 
-    intuition.
-  (*** MS END {"type": "proof", "proof_type":"manual"} *)
-  Restart.
-Proof.
-  (*** MS BEGIN {"type": "proof", "proof_type":"hammer", "total":2, "finished":0} *)
-  induction r.
-  - admit. (* hammer. *)
-  - admit. (* hammer. *)
-  (*** MS END {"type": "proof", "proof_type":"hammer", "total":2, "finished":0} *)
-  Restart.
-Proof.
-  (*** MS BEGIN {"type": "proof", "proof_type":"mirrorsolve", "total":2} *)
-  induction r;
-  mirrorsolve prep_proof.
-  (*** MS END {"type": "proof", "proof_type":"mirrorsolve", "total":2} *)
-Admitted.
+  (* Equations elements (t : tree) : list (key * V) := {
+    elements E := [] ;
+    elements (T l k v r) := elements l ++ [(k, v)] ++ elements r;
+  }. *)
 
-(*** MS BEGIN {"type": "configuration", "config_type":"tactics"} *)
-Ltac prep_proof' := Utils.pose_all (tt, insert_left_lt, insert_right_lt); 
-  prep_proof.
+(** Here are three desirable properties for [elements]:
 
-(*** MS END {"type": "configuration", "config_type":"tactics"} *)
+    1. The list has the same bindings as the tree.
 
-(*** MS BEGIN {"type": "proof_definition"} *)
-Lemma insert_ordered_left :
-  forall (l: tree V) k k' v, 
-    (k < k')%Z -> 
-    lt_t k' l -> 
-    ordered l ->
-    ordered (insert k v l).
-(*** MS END {"type": "proof_definition"} *)
-Proof.
-  (*** MS BEGIN {"type": "proof", "proof_type":"manual"} *)
-  induction l;
-  intros;
-  simpl in *.
-  - intuition.
-  - destruct (k0 <? k)%Z eqn:?;
-    simpl in *.
-    * intuition.
-      eapply insert_left_lt;
-      eauto.
-      Lia.lia.
-    * destruct (k0 >? k)%Z eqn:?;
-      simpl in *; 
-      intuition.
-      + eapply insert_right_lt;
-        intuition.
-      + assert (k0 = k) by Lia.lia.
-        subst.
-        trivial.
-      + assert (k0 = k) by Lia.lia.
-        subst.
-        trivial.
-  (*** MS END {"type": "proof", "proof_type":"manual"} *)
-  Restart.
-Proof.
-  (*** MS BEGIN {"type": "proof", "proof_type":"hammer", "total":2, "finished":1} *)
-  induction l.
-  (* - hammer.
-  - admit. *)
-  (*** MS END {"type": "proof", "proof_type":"hammer", "total":2, "finished":1} *)
-  Restart.
-Proof.
-  (*** MS BEGIN {"type": "proof", "proof_type":"mirrorsolve", "total":2} *)
-  induction l;
-  mirrorsolve prep_proof'.
-(*** MS END {"type": "proof", "proof_type":"mirrorsolve", "total":2} *)
-Admitted.
+    2. The list is sorted by keys.
 
-(*** MS BEGIN {"type": "proof_definition"} *)
-Lemma insert_ordered_right :
-forall (r: tree V) k k' v, 
-  (k > k')%Z -> 
-  gt_t k' r -> 
-  ordered r ->
-  ordered (insert k v r).
-(*** MS END {"type": "proof_definition"} *)
+    3. The list contains no duplicate keys.
+
+    Let's formally specify and verify them. *)
+
+(* ================================================================= *)
+(** ** Part 1: Same Bindings *)
+
+(** We want to show that a binding is in [elements t] iff it's in
+    [t]. We'll prove the two directions of that bi-implication
+    separately:
+
+    - [elements] is _complete_: if a binding is in [t] then it's in
+      [elements t].
+
+    - [elements] is _correct_: if a binding is in [elements t] then
+      it's in [t].  *)
+
+(** **** Exercise: 3 stars, standard (elements_complete) *)
+
+(** Prove that [elements] is complete. Proceed by induction on [t]. *)
+
+  Hint Immediate elements_equation_1 : tree_eqns.
+  Hint Immediate elements_equation_2 : tree_eqns.
+
+  Lemma In_nil : 
+    forall (x : key * V), 
+      In x [] <-> False.
+  Proof.
+    intuition eauto.
+  Qed.
+
+  Lemma In_cons : 
+    forall (x : key * V) x' xs, 
+      In x (x' :: xs) <-> (x = x' \/ In x xs).
+  Proof.
+    intros;
+    simpl in *;
+    intuition eauto.
+  Qed.
+
+  Hint Immediate In_cons : tree_eqns.
+  Hint Immediate In_nil : tree_eqns.
+
+  Lemma in_app_iff' :  
+    forall l l' (a:(key * V)), In a (l++l') <-> In a l \/ In a l'.
+  Proof.
+    eapply in_app_iff.
+  Qed.
+
+  Hint Immediate in_app_iff' : tree_eqns.
+
+  Theorem elements_complete : 
+    forall (t: tree) (k : key) (v d : V),
+      bound_t k t = true ->
+      lookup_t d k t = v ->
+      In (k, v) (elements t).
+  Proof.
+    induction t;
+    mirrorsolve.
+  Qed.
+
+  Hint Immediate elements_complete : tree_eqns.
+
+(** [] *)
+
+(** Proving correctness requires more work than completeness.
+
+    [BST] uses [ForallT] to say that all nodes in the left/right
+    subtree have smaller/greater keys than the root.  We need to
+    relate [ForallT], which expresses that all nodes satisfy a
+    property, to [Forall], which expresses that all list elements
+    satisfy a property.
+
+    The standard library contains a helpful lemma about [Forall]: *)
+
+Check Forall_app. 
+
+(** **** Exercise: 2 stars, standard (elements_preserves_forall) *)
+
+(** Prove that if a property [P] holds of every node in a tree [t],
+    then that property holds of every pair in [elements t]. Proceed
+    by induction on [t].
+
+    There is a little mismatch between the type of [P] in [ForallT]
+    and the type of the property accepted by [Forall], so we have to
+    _uncurry_ [P] when we pass it to [Forall]. (See [Poly] for
+    more about uncurrying.) The single quote used below is the Coq
+    syntax for doing a pattern match in the function arguments. *)
+
+Definition uncurry {X Y Z : Type} (f : X -> Y -> Z) '(a, b) :=
+  f a b.
+
+Hint Transparent uncurry.
+
+(* MIRRORSOLVE: We can't do this because of ForallT *)
+Lemma elements_preserves_forall : forall (P : key -> V -> Prop) (t : tree),
+    ForallT P t ->
+    Forall (uncurry P) (elements t).
 Proof.
-  (*** MS BEGIN {"type": "proof", "proof_type":"manual"} *)
-  induction r;
-  intros;
-  simpl in *.
-  - intuition.
-  - destruct (k0 <? k)%Z eqn:?;
-    simpl in *.
-    * intuition.
-      eapply insert_left_lt;
-      eauto.
-      Lia.lia.
-    * destruct (k0 >? k)%Z eqn:?;
-      simpl in *; 
-      intuition.
-      + eapply insert_right_lt;
-        intuition.
-      + assert (k0 = k) by Lia.lia.
-        subst.
-        trivial.
-      + assert (k0 = k) by Lia.lia.
-        subst.
-        trivial.
-  Restart.
-  (*** MS END {"type": "proof", "proof_type":"manual"} *)
+  (* FILL IN HERE *) Admitted.
+
+(** [] *)
+
+(** **** Exercise: 2 stars, standard (elements_preserves_relation) *)
+
+(** Prove that if all the keys in [t] are in a relation [R] with a
+    distinguished key [k'], then any key [k] in [elements t] is also
+    related by [R] to [k']. For example, [R] could be [<], in which
+    case the lemma says that if all the keys in [t] are less than
+    [k'], then all the keys in [elements t] are also less than
+    [k'].
+
+    Hint: you don't need induction.  Immediately look for a way
+    to use [elements_preserves_forall] and library theorem
+    [Forall_forall]. *)
+
+(* MIRRORSOLVE: We can't do this because it's higher-order *)
+Lemma elements_preserves_relation :
+  forall (k k' : key) (v : V) (t : tree) (R : key -> key -> Prop),
+    ForallT (fun y _ => R y k') t
+    -> In (k, v) (elements t)
+    -> R k k'.
 Proof.
-  (*** MS BEGIN {"type": "proof", "proof_type":"hammer", "total":2, "finished":1} *)
-  induction r.
-  (* - hammer.
-  - admit.  *)
-(*** MS END {"type": "proof", "proof_type":"hammer", "total":2, "finished":1} *)
-  Restart.
-Proof.
-  (*** MS BEGIN {"type": "proof", "proof_type":"mirrorsolve", "total":2} *)
-  induction r;
-  mirrorsolve prep_proof'.
-(*** MS END {"type": "proof", "proof_type":"mirrorsolve", "total":2} *)
-Admitted.
+  (* FILL IN HERE *) Admitted.
+
+
+  Lemma lt_list_nil : 
+    forall x, lt_list x [] <-> True.
+  Proof.
+    intros;
+    simpl in *;
+    intuition eauto.
+  Qed.
+
+  Lemma lt_list_cons : 
+    forall x y v l, lt_list x ((y, v) :: l)  <-> (y < x /\ lt_list x l).
+  Proof.
+    intros;
+    simpl in *;
+    intuition eauto.
+  Qed.
+
+  Lemma gt_list_nil : 
+    forall x, gt_list x [] <-> True.
+  Proof.
+    intros;
+    simpl in *;
+    intuition eauto.
+  Qed.
+
+  Lemma gt_list_cons : 
+    forall x y v l, gt_list x ((y, v) :: l)  <-> (y > x /\ gt_list x l).
+  Proof.
+    intros;
+    simpl in *;
+    intuition eauto.
+  Qed.
+
+  Hint Immediate lt_list_nil : tree_eqns.
+  Hint Immediate lt_list_cons : tree_eqns.
+  Hint Immediate gt_list_nil : tree_eqns.
+  Hint Immediate gt_list_cons : tree_eqns.
+
+  (* However, we can prove that it preserves lt_t and gt_t, as well as that lt_list and gt_list are transitive *)
+
+  Lemma lt_list_trans : 
+    forall l x y,
+      x < y -> 
+      lt_list x l -> 
+      lt_list y l.
+  Proof.
+    induction l;
+    mirrorsolve.
+  Qed.
+
+  Lemma gt_list_trans : 
+    forall l x y,
+      x > y -> 
+      gt_list x l -> 
+      gt_list y l.
+  Proof.
+    induction l;
+    mirrorsolve.
+  Qed.
+
+  Hint Immediate lt_list_trans : tree_eqns.
+  Hint Immediate gt_list_trans : tree_eqns.
+
+  SetSMTSolver "z3".
+
+  Lemma lt_list_In : 
+    forall x l, 
+      lt_list x l <-> (forall y v, In (y, v) l -> y < x).
+  Proof.
+    induction l;
+    mirrorsolve.
+  Qed.
+
   
-(*** MS BEGIN {"type": "configuration", "config_type":"tactics"} *)
-Ltac prep_proof'' := Utils.pose_all (tt, insert_ordered_left, insert_ordered_right);
-  prep_proof'.
-(*** MS END {"type": "configuration", "config_type":"tactics"} *)
 
-(*** MS BEGIN {"type": "proof_definition"} *)
-Theorem insert_ordered : 
-forall (t: tree V) k v,
-  ordered t -> 
-  ordered (insert k v t).
-(*** MS END {"type": "proof_definition"} *)
+  Lemma gt_list_In : 
+    forall x l, 
+      gt_list x l <-> (forall y v, In (y, v) l -> y > x).
+  Proof.
+    induction l;
+    mirrorsolve.
+  Qed.
+
+  Hint Immediate lt_list_In : tree_eqns.
+  Hint Immediate gt_list_In : tree_eqns.
+
+
+  Lemma lt_t_elements : 
+    forall t x,
+      lt_t x t <-> lt_list x (elements t).
+  Proof.
+    induction t;
+    try mirrorsolve.
+  Qed.
+
+  Lemma gt_t_elements : 
+    forall t x,
+      gt_t x t <-> gt_list x (elements t).
+  Proof.
+    induction t;
+    try mirrorsolve.
+  Qed.
+
+  Hint Immediate lt_t_elements : tree_eqns.
+  Hint Immediate gt_t_elements : tree_eqns.
+
+
+(** [] *)
+
+(** **** Exercise: 4 stars, standard (elements_correct) *)
+
+(** Prove that [elements] is correct. Proceed by induction on the
+    evidence that [t] is a BST. *)
+
+  Theorem elements_correct : 
+    forall (t : tree) (k : key) (v d : V),
+      BST t ->
+      In (k, v) (elements t) ->
+      bound_t k t = true /\ lookup_t d k t = v.
+  Proof.
+    induction t;
+    mirrorsolve.
+  Qed.
+
+  Hint Immediate elements_correct : tree_eqns.
+
+(** [] *)
+
+(** The inverses of completeness and correctness also should hold:
+
+    - inverse completeness: if a binding is not in [t] then it's not
+      in [elements t].
+
+    - inverse correctness: if a binding is not in [elements t] then
+      it's not in [t].
+
+    Let's prove that they do. *)
+
+(** **** Exercise: 2 stars, advanced (elements_complete_inverse) *)
+
+(** This inverse doesn't require induction.  Look for a way to use
+    [elements_correct] to quickly prove the result. *)
+
+  Theorem elements_complete_inverse :
+    forall (t : tree) (k : key) (v : V) ,
+      BST t -> 
+      bound_t k t = false ->
+      ~ In (k, v) (elements t).
+  Proof.
+    induction t;
+    mirrorsolve.
+  Qed.
+
+  Hint Immediate elements_complete_inverse : tree_eqns.
+
+(** [] *)
+
+(** **** Exercise: 4 stars, advanced (elements_correct_inverse) *)
+
+(** Prove the inverse.  First, prove this helper lemma by induction on
+    [t]. *)
+
+(* We can't prove this because there's an exists *)
+Lemma bound_value : forall (k : key) (t : tree),
+    bound_t k t = true -> exists v, forall d, lookup_t d k t = v.
 Proof.
-  (*** MS BEGIN {"type": "proof", "proof_type":"manual"} *)
-  induction t;
-  intros;
-  simpl in *.
-  - intuition.
-  - destruct (k0 <? k)%Z eqn:?;
-    simpl in *.
-    * intuition.
-      eapply insert_left_lt;
-      intuition.
-    * destruct (k0 >? k)%Z eqn:?;
-      simpl in *; 
-      intuition.
-      + eapply insert_right_lt;
-        intuition.
-      + assert (k0 = k) by Lia.lia.
-        subst.
-        trivial.
-      + assert (k0 = k) by Lia.lia.
-        subst.
-        trivial.
-(*** MS END {"type": "proof", "proof_type":"manual"} *)
-  Restart.
+  (* FILL IN HERE *) Admitted.
+
+(** Prove the main result.  You don't need induction. *)
+
+  Theorem elements_correct_inverse :
+    forall (t : tree) (k : key) ,
+      (forall v, ~ In (k, v) (elements t)) ->
+      bound_t k t = false.
+  Proof.
+    induction t;
+    mirrorsolve.
+  Qed.
+
+  Hint Immediate elements_correct_inverse : tree_eqns.
+
+  
+(* ================================================================= *)
+(** ** Part 2: Sorted (Advanced) *)
+
+(** We want to show that [elements] is sorted by keys.  We follow a
+    proof technique contributed by Lydia Symmons et al.*)
+
+(** **** Exercise: 3 stars, advanced (sorted_app) *)
+
+  (* First we reflect the definition of sorted to UF: *)
+
+  Lemma sorted_nil' : 
+    sorted [] <-> True.
+  Proof.
+    intros;
+    simpl;
+    intuition eauto.
+    econstructor.
+  Qed.
+
+  Lemma sorted_one' :
+    forall x, 
+    sorted [x] <-> True.
+  Proof.
+    intros;
+    simpl;
+    intuition eauto.
+    econstructor.
+  Qed.
+
+  Lemma sorted_cons' : 
+    forall (x y : key) (l : list key),
+      sorted (x :: y :: l) <-> (x <= y /\ sorted (y :: l)).
+  Proof.
+    intros;
+    simpl;
+    intuition eauto;
+    try match goal with 
+    | H: sorted (_ :: _ :: _) |- _ => inversion H; subst
+    end;
+    eauto.
+    econstructor;
+    eauto.
+  Qed.
+
+  Hint Immediate sorted_nil' : tree_eqns.
+  Hint Immediate sorted_one' : tree_eqns.
+  Hint Immediate sorted_cons' : tree_eqns.
+
+  Lemma lt_list_s_nil : 
+    forall x, lt_list_s x [] <-> True.
+  Proof.
+    intros;
+    simpl in *;
+    intuition eauto.
+  Qed.
+
+  Lemma lt_list_s_cons : 
+    forall l x y, lt_list_s x (y :: l)  <-> (y < x /\ lt_list_s x l).
+  Proof.
+    intros;
+    simpl in *;
+    intuition eauto.
+  Qed.
+
+  Hint Immediate lt_list_s_nil : tree_eqns.
+  Hint Immediate lt_list_s_cons : tree_eqns.
+  
+  Lemma app_nil_l_Z : 
+    forall (x: list key), ([] ++ x = x)%list.
+  Proof.
+    eapply app_nil_l.
+  Qed.
+
+  Lemma app_cons_l_Z : 
+    forall (x: key) y z, ((x :: y) ++ z = x :: (y ++ z))%list.
+  Proof.
+    intros;
+    intuition eauto.
+  Qed.
+
+  Hint Immediate app_nil_l_Z : tree_eqns.
+  Hint Immediate app_cons_l_Z : tree_eqns.
+
+  Lemma sorted_lt_end : 
+    forall l x, 
+      lt_list_s x l -> 
+      sorted l -> 
+      sorted (l ++ [x]).
+  Proof.
+    
+    induction l;
+    try mirrorsolve.
+  Qed.
+
+  Hint Immediate sorted_lt_end : tree_eqns.
+
+  Lemma gt_list_s_nil : 
+    forall x, gt_list_s x [] <-> True.
+  Proof.
+    intros;
+    simpl in *;
+    intuition eauto.
+  Qed.
+
+  Lemma gt_list_s_cons : 
+    forall l x y, gt_list_s x (y :: l)  <-> (y > x /\ gt_list_s x l).
+  Proof.
+    intros;
+    simpl in *;
+    intuition eauto.
+  Qed.
+
+  Hint Immediate gt_list_s_nil : tree_eqns.
+  Hint Immediate gt_list_s_cons : tree_eqns.
+
+  Lemma sorted_gt_beginning : 
+    forall r x, 
+      gt_list_s x r -> 
+      sorted r -> 
+      sorted (x :: r).
+  Proof.
+    induction r;
+    mirrorsolve.
+  Qed.
+
+  Hint Immediate sorted_gt_beginning : tree_eqns.
+
+
+(** Prove that inserting an intermediate value between two lists
+    maintains sortedness. Proceed by induction on the evidence
+    that [l1] is sorted. *)
+
+(* We can't prove this because of Forall, but we can replace Forall and prove something about that *)
+  Lemma sorted_app: forall l1 l2 x,
+    sorted l1 -> sorted l2 ->
+    Forall (fun n => n < x) l1 -> Forall (fun n => n > x) l2 ->
+    sorted (l1 ++ x :: l2).
+  Proof.
+    (* FILL IN HERE *) Admitted.
+
+  Lemma sorted_app': forall l1 l2 x,
+   sorted l1 ->sorted l2 ->
+    lt_list_s x l1 -> gt_list_s x l2 ->
+   sorted (l1 ++ x :: l2).
+  Proof.
+    induction l1;
+    induction l2;
+    mirrorsolve.
+  Qed.
+
+  Hint Immediate sorted_app' : tree_eqns.
+
+(** [] *)
+
+(** **** Exercise: 4 stars, advanced (sorted_elements) *)
+
+(** The keys in an association list are the first elements of every
+    pair: *)
+
+  Definition list_keys (lst : list (key * V)) :=
+    map fst lst.
+
+(** Prove that [elements t] is sorted by keys. Proceed by induction
+    on the evidence that [t] is a BST. *)
+
+  (* We can't directly prove this because of map, but we can replace it with map_fst *)
+  Theorem sorted_elements : forall (t : tree),
+      BST t -> sorted (list_keys (elements t)).
+  Proof.
+  (* FILL IN HERE *) Admitted.
+
+  Hint Immediate map_fst_equation_1 : tree_eqns.
+  Hint Immediate map_fst_equation_2 : tree_eqns.
+
+  Lemma map_fst_lts : 
+    forall l x, 
+      lt_list x l <-> lt_list_s x (map_fst l).
+  Proof.
+    induction l;
+    mirrorsolve. 
+  Qed.
+
+  Lemma map_fst_gts : 
+    forall l x, 
+      gt_list x l <-> gt_list_s x (map_fst l).
+  Proof.
+    induction l;
+    mirrorsolve. 
+  Qed.
+
+  Hint Immediate map_fst_lts : tree_eqns.
+  Hint Immediate map_fst_gts : tree_eqns.
+
+  Lemma app_nil_l_Z_V : 
+    forall (x: list (key * V)), ([] ++ x = x)%list.
+  Proof.
+    eapply app_nil_l.
+  Qed.
+
+  Lemma app_cons_l_Z_V : 
+    forall (x: (key * V)) y z, ((x :: y) ++ z = x :: (y ++ z))%list.
+  Proof.
+    intros;
+    intuition eauto.
+  Qed.
+
+  Hint Immediate app_nil_l_Z_V : tree_eqns.
+  Hint Immediate app_cons_l_Z_V : tree_eqns.
+
+  SetSMTSolver "cvc5".
+
+  Lemma map_fst_app :
+    forall x y, 
+      (map_fst (x ++ y) = map_fst x ++ map_fst y)%list.
+  Proof.
+    induction x; 
+    mirrorsolve.
+  Qed. 
+
+  Hint Immediate map_fst_app : tree_eqns.
+
+  Theorem sorted_elements' : forall (t : tree),
+      BST t -> sorted (map_fst (elements t)).
+  Proof.
+    induction t;
+    mirrorsolve.
+  Qed.
+
+  Hint Resolve sorted_elements' : tree_eqns.
+
+(** [] *)
+
+(* ================================================================= *)
+(** ** Part 3: No Duplicates (Advanced and Optional) *)
+
+(** We want to show that [elements t] contains no duplicate
+    key bindings. Tree [t] itself cannot contain any duplicates, so the
+    list that [elements] produces shouldn't either. The standard
+    library already contains a helpful inductive proposition,
+    [NoDup]. *)
+
+(** The library is missing a theorem, though, about [NoDup] and [++].
+    To state that theorem, we first need to formalize what it means
+    for two lists to be disjoint: *)
+
+  Hint Immediate disjoint_spec : tree_eqns.
+  Hint Immediate nd_z_nil : tree_eqns.
+  Hint Immediate nd_z_cons : tree_eqns.
+
+  Lemma In_nil_Z : 
+    forall (x : key), 
+      In x [] <-> False.
+  Proof.
+    intros;
+    simpl in *;
+    intuition eauto.
+  Qed.
+
+  Lemma In_cons_Z : 
+    forall (x : key) x' xs, 
+      In x (x' :: xs) <-> (x = x' \/ In x xs).
+  Proof.
+    intros;
+    simpl in *;
+    intuition eauto.
+  Qed.
+
+  Hint Immediate In_cons_Z : tree_eqns.
+  Hint Immediate In_nil_Z : tree_eqns.
+
+(** **** Exercise: 3 stars, advanced, optional (NoDup_append) *)
+
+(** Prove that if two lists are disjoint, appending them preserves
+    [NoDup].  Hint: You might already have proved this theorem in an
+    advanced exercise in [IndProp]. *)
+
+  Lemma disjoint_cons: 
+    forall x l r, 
+      disjoint (x :: l) r -> disjoint l r.
+  Proof.
+    induction l;
+    mirrorsolve.
+  Qed.
+  
+  Hint Immediate disjoint_cons : tree_eqns.
+
+  Lemma neg_In_app : 
+    forall (x: Z) l r, 
+      ~ In x l -> ~ In x r -> ~ In x (l ++ r).
+  Proof.
+    induction l;
+    mirrorsolve.
+  Qed.
+
+  Hint Immediate neg_In_app : tree_eqns.
+
+
+
+  Lemma NoDup_append : forall (l1 l2: list Z),
+    NoDup_Z l1 -> NoDup_Z l2 -> disjoint l1 l2 ->
+    NoDup_Z (l1 ++ l2).
+  Proof.
+    induction l1;
+    mirrorsolve.
+  Qed.
+
+  Hint Immediate NoDup_append : tree_eqns.
+
+  Lemma Not_In_nil : 
+    forall (x: key), ~ In x [].
+  Proof.
+    mirrorsolve.
+  Qed.
+
+  Lemma Not_In_cons:
+    forall l (x: key) x', 
+      ~ In x (x' :: l) <-> (x <> x' /\ ~ In x l).
+  Proof.
+    induction l;
+    mirrorsolve.
+  Qed.
+
+  Hint Immediate Not_In_nil : tree_eqns.
+  Hint Immediate Not_In_cons : tree_eqns.
+
+  Lemma gt_t_notin : 
+    forall l x, 
+      gt_list_s x l -> ~ In x l.
+  Proof.
+    induction l;
+    mirrorsolve.
+  Qed.
+
+  Lemma lt_t_notin : 
+    forall l x, 
+      lt_list_s x l -> ~ In x l.
+  Proof.
+    induction l;
+    mirrorsolve.
+  Qed.
+
+  Hint Immediate gt_t_notin : tree_eqns.
+  Hint Immediate lt_t_notin : tree_eqns.
+
+
+  Lemma gt_t_disjoint : 
+    forall l2 l1, 
+      (forall x, In x l1 -> 
+      gt_list_s x l2) -> 
+      disjoint l1 l2.
+  Proof.
+    mirrorsolve.
+  Qed.
+
+  Lemma lt_t_disjoint : 
+    forall l2 l1, 
+      (forall x, In x l1 -> 
+      lt_list_s x l2) -> 
+      disjoint l1 l2.
+  Proof.
+    mirrorsolve.
+  Qed.
+  
+  Hint Immediate lt_t_disjoint : tree_eqns.
+  Hint Immediate gt_t_disjoint : tree_eqns.
+
+(** [] *)
+
+(** **** Exercise: 4 stars, advanced, optional (elements_nodup_keys) *)
+
+(** Prove that there are no duplicate keys in the list returned
+    by [elements]. Proceed by induction on the evidence that [t] is a
+    BST. Make use of library theorems about [map] as needed. *)
+
+    (* We can't prove this because it uses map and nodup, but we can prove one with map_fst and nodup_z! *)
+  Theorem elements_nodup_keys : forall (t : tree),
+    BST t ->
+    NoDup (list_keys (elements t)).
+  Proof.
+  (* FILL IN HERE *) Admitted.
+
+  Theorem elements_nodup_keys' : forall (t : tree),
+    ordered t ->
+    NoDup_Z (map_fst (elements t)).
+  Proof.
+    induction t;
+    mirrorsolve.
+  Qed.
+
+  Hint Immediate elements_nodup_keys' : tree_eqns.
+
+(** [] *)
+
+(** That concludes the proof of correctness of [elements]. *)
+
+(* ################################################################# *)
+(** * A Faster [elements] Implementation *)
+
+
+  Hint Immediate fast_elements_tr_equation_1 : tree_eqns.
+  Hint Immediate fast_elements_tr_equation_2 : tree_eqns.
+
+(** The implemention of [elements] is inefficient because of how
+    it uses the [++] operator.  On a balanced tree its running time is
+    linearithmic, because it does a linear number of concatentations
+    at each level of the tree. On an unbalanced tree it's quadratic
+    time.  Here's a tail-recursive implementation than runs in linear
+    time, regardless of whether the tree is balanced: *)
+
+(** **** Exercise: 3 stars, standard (fast_elements_eq_elements) *)
+
+(** Prove that [fast_elements] and [elements] compute the same
+    function. *)
+
+  Lemma app_comm_K_Z : 
+    forall (x: list (key * V)) y z, 
+      (x ++ y ++ z = (x ++ y) ++ z)%list.
+  Proof.
+    induction x;
+    mirrorsolve.
+  Qed.
+
+  Hint Immediate app_comm_K_Z : tree_eqns.
+
+  Lemma fast_elements_tr_helper :
+    forall (t : tree) (lst : list (key * V)),
+      (fast_elements_tr t lst = elements t ++ lst)%list.
+  Proof.
+    induction t;
+    mirrorsolve.
+  Qed.
+
+  Hint Immediate fast_elements_tr_helper : tree_eqns.
+
+  Lemma app_nil_r_K_V:
+    forall (x: list (key * V)), (x ++ [] = x)%list.
+  Proof.
+    induction x;
+    mirrorsolve.
+  Qed.
+
+  Hint Immediate app_nil_r_K_V : tree_eqns.
+
+  Hint Immediate fast_elements_equation_1 : tree_eqns.
+  Lemma fast_elements_eq_elements : forall (t : tree),
+      fast_elements t = elements t.
+  Proof.
+    mirrorsolve.
+  Qed.
+
+  Hint Immediate fast_elements_eq_elements : tree_eqns.
+
+
+(** [] *)
+
+(** Since the two implementations compute the same function, all
+    the results we proved about the correctness of [elements]
+    also hold for [fast_elements].  For example: *)
+
+  Corollary fast_elements_correct :
+    forall (t: tree) (k : key) (v d : V),
+      BST t ->
+      In (k, v) (fast_elements t) ->
+      bound_t k t = true /\ lookup_t d k t = v.
+  Proof.
+    mirrorsolve.
+  Qed.
+
+(** This corollary illustrates a general technique:  prove the correctness
+    of a simple, slow implementation; then prove that the slow version
+    is functionally equivalent to a fast implementation.  The proof of
+    correctness for the fast implementation then comes "for free". *)
+
+(* ################################################################# *)
+(** * An Algebraic Specification of [elements] *)
+
+(** The verification of [elements] we did above did not adhere to the
+    algebraic specification approach, which would suggest that we look
+    for equations of the form
+
+      elements empty_tree = ...
+      elements (insert k v t) = ... (elements t) ...
+
+    The first of these is easy; we can trivially prove the following:
+    *)
+
+  Lemma elements_empty :
+      elements empty_tree = [].
+  Proof.
+    mirrorsolve.
+  Qed.
+
+(** But for the second equation, we have to express the result of
+    inserting [(k, v)] into the elements list for [t], accounting for
+    ordering and the possibility that [t] may already contain a pair
+    [(k, v')] which must be replaced.  The following rather ugly
+    function will do the trick: *)
+
+(** That's not satisfactory, because the definition of
+    [kvs_insert] is so complex. Moreover, this equation doesn't tell
+    us anything directly about the overall properties of [elements t]
+    for a given tree [t].  Nonetheless, we can proceed with a rather
+    ugly verification. *)
+
+(* MIRRORSOLVE: We can't do this one because it uses Forall, but we can prove an equivalent version with lt/gt_list. *)
+
+  (** **** Exercise: 3 stars, standard, optional (kvs_insert_split) *)
+  Lemma kvs_insert_split :
+    forall (v v0 : V) (e1 e2 : list (key * V)) (k k0 : key),
+      (Forall (fun '(k',_) => k' < k0) e1 ->
+      Forall (fun '(k',_) => k' > k0) e2 ->
+      kvs_insert k v (e1 ++ (k0,v0):: e2) =
+      if k <? k0 then
+        (kvs_insert k v e1) ++ (k0,v0)::e2
+      else if k >? k0 then
+            e1 ++ (k0,v0)::(kvs_insert k v e2)
+          else
+            e1 ++ (k,v)::e2)%list.
+  Proof.
+  (* FILL IN HERE *) Admitted.
+  (** [] *)
+
+  Hint Immediate kvs_insert_equation_1 : tree_eqns.
+  Hint Immediate kvs_insert_equation_2 : tree_eqns.
+
+  Lemma kvs_insert_split' :
+    forall (e1 e2 : list (key * V)) (v v0 : V) (k k0 : key),
+      (lt_list k0 e1 -> 
+      gt_list k0 e2 ->
+      kvs_insert k v (e1 ++ (k0,v0):: e2) =
+      ite (k <? k0) 
+        ((kvs_insert k v e1) ++ (k0,v0)::e2) (
+      ite (k >? k0) 
+        (e1 ++ (k0,v0)::(kvs_insert k v e2)) (
+        (e1 ++ (k,v)::e2))))%list.
+  Proof.
+    induction e1;
+    induction e2;
+    mirrorsolve.
+  Qed.
+
+  Hint Immediate kvs_insert_split' : tree_eqns.
+  (** **** Exercise: 3 stars, standard, optional (kvs_insert_elements) *)
+  Lemma kvs_insert_elements : forall (t : tree),
+      BST t ->
+      forall (k : key) (v : V),
+        elements (insert_t k v t) = kvs_insert k v (elements t).
+  Proof.
+    induction t;
+    mirrorsolve.
+  Qed.
+
+
+(* MIRRORSOLVE: We can't do any of these specs because they use functional maps.
+   Although maybe there is a clever way to represent functional maps in SMT.
+  *)
+
+(* ################################################################# *)
+(** * Model-based Specifications *)
+
+(** At the outset, we mentioned studying two techniques for
+    specifying the correctness of BST operations in this chapter.  The
+    first was algebraic specification.
+
+    Another approach to proving correctness of search trees is to
+    relate them to our existing implementation of functional partial
+    maps, as developed in [Maps]. To prove the correctness of a
+    search-tree algorithm, we can prove:
+
+    - Any search tree corresponds to some functional partial map,
+      using a function or relation that we write down.
+
+    - The [lookup] operation on trees gives the same result as the
+      [find] operation on the corresponding map.
+
+    - Given a tree and corresponding map, if we [insert] on the tree
+      and [update] the map with the same key and value, the resulting
+      tree and map are in correspondence.
+
+    This approach is sometimes called _model-based specification_: we
+    show that our implementation of a data type corresponds to a more
+    more abstract _model_ type that we already understand. To reason
+    about programs that use the implementation, it suffices to reason
+    about the behavior of the abstract type, which may be
+    significantly easier.  For example, we can take advantage of laws
+    that we proved for the abstract type, like [update_eq] for
+    functional maps, without having to prove them again for the
+    concrete tree type.
+
+    We also need to be careful here, because the type of functional
+    maps as defined in [Maps] do not actually behave quite like
+    our tree-based maps. For one thing, functional maps can be defined
+    on an infinite number of keys, and there is no mechanism for
+    enumerating over the key set. To maintain correspondence with our
+    finite trees, we need to make sure that we consider only
+    functional maps built by finitely many applications of constructor
+    functions ([empty] and [update]). Also, thanks to functional
+    extensionality, functional maps obey stronger equality laws than
+    our trees do (as we investigated in the [direct_equalities]
+    exercise above), so we should not be misled into thinking that
+    every fact we can prove about abstract maps necessarily holds for
+    concrete ones.
+
+    Compared to the algebraic-specification approach described earlier
+    in this chapter, the model-based approach can save some proof
+    effort, especially if we already have a well-developed theory for
+    the abstract model type.  On the other hand, we have to give an
+    explicit _abstraction_ relation between trees and maps, and show
+    that it is maintained by all operations. In the end, about the
+    same amount of work is needed to show correctness, though the work
+    shows up in different places depending on how the abstraction
+    relation is defined. *)
+
+(** We now give a model-based specification for trees in terms
+    of functional partial maps. It is based on a simple abstraction
+    relation that builds a functional map element by element. *)
+
+  (* Fixpoint map_of_list {V : Type} (el : list (key * V)) : partial_map V :=
+    match el with
+    | [] => empty
+    | (k, v) :: el' => update (map_of_list el') k v
+    end.
+
+  Definition Abs {V : Type} (t : tree V) : partial_map V :=
+    map_of_list (elements t). *)
+
+(** In general, model-based specifications may use an abstraction
+    relation, allowing each concrete value to be related to multiple
+    abstract values.  But in this case a simple abstraction _function_
+    will do, assigning a unique abstract value to each concrete
+    one. *)
+
+(** One small difference between trees and functional maps is that
+    applying the latter returns an [option V] which might be [None],
+    whereas [lookup] returns a default value if key is not bound
+    lookup fails.  We can easily provide a function on functional
+    partial maps having the latter behavior. *)
+
+(* Definition find {V : Type} (d : V) (k : key) (m : partial_map V) : V :=
+  match m k with
+  | Some v => v
+  | None => d
+  end. *)
+
+(** We also need a [bound] operation on maps. *)
+
+(* Definition map_bound {V : Type} (k : key) (m : partial_map V) : bool :=
+  match m k with
+  | Some _ => true
+  | None => false
+  end. *)
+
+(** We now proceed to prove that each operation preserves (or establishes)
+    the abstraction relationship in an appropriate way:
+
+    concrete        abstract
+    --------        --------
+    empty_tree      empty
+    bound           map_bound
+    lookup          find
+    insert          update
+*)
+
+(** The following lemmas will be useful, though you are not required
+    to prove them. They can all be proved by induction on the list. *)
+
+(** **** Exercise: 2 stars, standard, optional (in_fst) *)
+(* Lemma in_fst : forall (X Y : Type) (lst : list (X * Y)) (x : X) (y : Y),
+    In (x, y) lst -> In x (map fst lst).
+Proof. *)
+  (* FILL IN HERE *)
+(** [] *)
+
+(** **** Exercise: 2 stars, standard, optional (in_map_of_list) *)
+(* Lemma in_map_of_list : forall (V : Type) (el : list (key * V)) (k : key) (v : V),
+    NoDup (map fst el) ->
+    In (k,v) el -> (map_of_list el) k = Some v.
+Proof. *)
+(* FILL IN HERE *)
+(** [] *)
+
+(** **** Exercise: 2 stars, standard, optional (not_in_map_of_list) *)
+(* Lemma not_in_map_of_list : forall (V : Type) (el : list (key * V)) (k : key),
+    ~ In k (map fst el) -> (map_of_list el) k = None.
+Proof. *)
+  (* FILL IN HERE *)
+(** [] *)
+
+(* Lemma empty_relate : forall (V : Type),
+    @Abs V empty_tree = empty.
 Proof.
-  (*** MS BEGIN {"type": "proof", "proof_type":"hammer", "total":2, "finished":1} *)
-  induction t.
-  (* - hammer.
-  - admit.  *)
-(*** MS END {"type": "proof", "proof_type":"hammer", "total":2, "finished":1} *)
-  Restart.
+  reflexivity.
+Qed. *)
+
+(** **** Exercise: 3 stars, standard, optional (bound_relate) *)
+
+(* Theorem bound_relate : forall (V : Type) (t : tree V) (k : key),
+    BST t ->
+    map_bound k (Abs t) = bound k t.
+Proof. *)
+  (* FILL IN HERE *)
+
+(** [] *)
+
+(** **** Exercise: 3 stars, standard, optional (lookup_relate) *)
+
+(* Lemma lookup_relate : forall (V : Type) (t : tree V) (d : V) (k : key),
+    BST t -> find d k (Abs t) = lookup d k t.
+Proof. *)
+  (* FILL IN HERE *)
+(** [] *)
+
+(** **** Exercise: 3 stars, standard, optional (insert_relate) *)
+(*
+Lemma insert_relate : forall (V : Type) (t : tree V) (k : key) (v : V),
+  BST t -> Abs (insert k v t) = update (Abs t) k v.
 Proof.
-  (*** MS BEGIN {"type": "proof", "proof_type":"mirrorsolve", "total":2} *)
-  induction t;
-  mirrorsolve prep_proof''.
-(*** MS END {"type": "proof", "proof_type":"mirrorsolve", "total":2} *)
-Admitted.
+  (* TODO: find a direct proof that doesn't rely on [kvs_insert_elements] *)
+    unfold Abs.
+  intros.
+  rewrite kvs_insert_elements; auto.
+  remember (elements t) as l.
+  clear -l. 
+  (* clear everything not about [l] *)
+  (* Hint: proceed by induction on [l]. *)
+    (* FILL IN HERE *)
+    *)
+(** [] *)
+
+(** The previous three lemmas are in essence saying that the following
+    diagrams commute.
+
+             bound k
+      t -------------------+
+      |                    |
+  Abs |                    |
+      V                    V
+      m -----------------> b
+           map_bound k
+
+            lookup d k
+      t -----------------> v
+      |                    |
+  Abs |                    | Some
+      V                    V
+      m -----------------> Some v
+             find d k
+
+            insert k v
+      t -----------------> t'
+      |                    |
+  Abs |                    | Abs
+      V                    V
+      m -----------------> m'
+            update' k v
+
+    Where we define:
+
+      update' k v m = update m k v
+
+*)
+
+(** Functional partial maps lack a way to extract or iterate
+    over their elements, so we cannot give an analogous abstract
+    operation for [elements]. Instead, we can prove this trivial
+    little lemma. *)
+
+(* Lemma elements_relate : forall (V : Type) (t : tree V),
+  BST t ->
+  map_of_list (elements t) = Abs t.
+Proof.
+  unfold Abs. intros. reflexivity.
+Qed. *)
+
+(* ################################################################# *)
+(** * An Alternative Abstraction Relation (Optional, Advanced) *)
+
+(** There is often more than one way to specify a suitable abstraction
+    relation between given concrete and abstract datatypes. The
+    following exercises explore another way to relate search trees to
+    functional partial maps without using [elements] as an
+    intermediate step.
+
+    We extend our definition of functional partial maps by adding a
+    new primitive for combining two partial maps, which we call
+    [union].  Our intention is that it only be used to combine maps
+    with disjoint key sets; to keep the operation symmetric, we make
+    the result be undefined on any key they have in common.  *)
+
+(* Definition union {X} (m1 m2: partial_map X) : partial_map X :=
+  fun k =>
+    match (m1 k, m2 k) with
+    | (None, None) => None
+    | (None, Some v) => Some v
+    | (Some v, None) => Some v
+    | (Some _, Some _) => None
+    end. *)
+
+(** We can prove some simple properties of lookup and update on unions,
+    which will prove useful later. *)
+
+(** **** Exercise: 2 stars, standard, optional (union_collapse) *)
+(* Lemma union_left : forall {X} (m1 m2: partial_map X) k,
+    m2 k = None -> union m1 m2 k = m1 k.
+Proof. 
+(* FILL IN HERE *) *)
+
+(* Lemma union_right : forall {X} (m1 m2: partial_map X) k,
+    m1 k = None ->
+    union m1 m2 k = m2 k.
+Proof.
+(* FILL IN HERE *) *)
+
+(* Lemma union_both : forall {X} (m1 m2 : partial_map X) k v1 v2,
+    m1 k = Some v1 ->
+    m2 k = Some v2 ->
+    union m1 m2 k = None.
+Proof.
+(* FILL IN HERE *) *)
+(** [] *)
+
+(** **** Exercise: 3 stars, standard, optional (union_update) *)
+(* Lemma union_update_right : forall {X} (m1 m2: partial_map X) k v,
+    m1 k = None ->
+    update (union m1 m2) k v = union m1 (update m2 k v).
+Proof.
+(* FILL IN HERE *) *)
+
+(* Lemma union_update_left : forall {X} (m1 m2: partial_map X) k v,
+    m2 k = None ->
+    update (union m1 m2) k v = union (update m1 k v) m2.
+Proof.
+(* FILL IN HERE *) *)
+(** [] *)
+
+(** We can now write a direct conversion function from trees to maps
+    based on the structure of the tree, and prove a basic property
+    preservation result. *)
+
+(* Fixpoint map_of_tree {V : Type} (t: tree V) : partial_map V :=
+  match t with
+  | E => empty
+  | T l k v r => update (union (map_of_tree l) (map_of_tree r)) k v
+  end. *)
+
+(** **** Exercise: 3 stars, advanced, optional (map_of_tree_prop) *)
+(* Lemma map_of_tree_prop : forall (V : Type) (P : key -> V -> Prop) (t : tree V),
+    ForallT P t ->
+    forall k v, (map_of_tree t) k = Some v ->
+           P k v.
+Proof.
+  (* FILL IN HERE *) *)
+(** [] *)
+
+(** Finally, we define our new abstraction function, and prove the
+    same lemmas as before. *)
+
+(* Definition Abs' {V : Type} (t: tree V) : partial_map V :=
+  map_of_tree t.
+
+Lemma empty_relate' : forall (V : Type),
+    @Abs' V empty_tree = empty.
+Proof.
+  reflexivity.
+Qed. *)
+
+(** **** Exercise: 3 stars, advanced, optional (bound_relate') *)
+(* Theorem bound_relate' : forall (V : Type) (t : tree V) (k : key),
+    BST t ->
+    map_bound k (Abs' t) = bound k t.
+Proof.
+  (* FILL IN HERE *) *)
+(** [] *)
+
+(** **** Exercise: 3 stars, advanced, optional (lookup_relate') *)
+(* Lemma lookup_relate' : forall (V : Type) (d : V) (t : tree V) (k : key),
+    BST t -> find d k (Abs' t) = lookup d k t.
+Proof.
+  (* FILL IN HERE *) *)
+(** [] *)
+
+(** **** Exercise: 4 stars, advanced, optional (insert_relate') *)
+(* Lemma insert_relate' : forall (V : Type) (k : key) (v : V) (t : tree V),
+   BST t -> Abs' (insert k v t) = update (Abs' t) k v.
+Proof.
+  (* FILL IN HERE *) *)
+(** [] *)
+
+(** The [elements_relate] lemma, which was trivial for our previous [Abs]
+    function, is considerably harder this time.  We suggest starting with
+    an auxiliary lemma. *)
+
+(** **** Exercise: 3 stars, advanced, optional (map_of_list_app) *)
+(* Lemma map_of_list_app : forall (V : Type) (el1 el2: list (key * V)),
+   disjoint (map fst el1) (map fst el2) ->
+   map_of_list (el1 ++ el2) = union (map_of_list el1) (map_of_list el2).
+Proof.
+  (* FILL IN HERE *) *)
+(** [] *)
+
+(** **** Exercise: 4 stars, advanced, optional (elements_relate') *)
+(* Lemma elements_relate' : forall (V : Type) (t : tree V),
+  BST t ->
+  map_of_list (elements t) = Abs' t.
+Proof.
+  (* FILL IN HERE *) *)
+(** [] *)
+
+(* ################################################################# *)
+(** * Efficiency of Search Trees *)
+
+(** All the theory we've developed so far has been about correctness.
+    But the reason we use binary search trees is that they are
+    efficient.  That is, if there are [N] elements in a (reasonably
+    well balanced) BST, each insertion or lookup takes about [log N]
+    time.
+
+    What could go wrong?
+
+     1. The search tree might not be balanced.  In that case, each
+        insertion or lookup will take as much as linear time.
+
+        - SOLUTION: use an algorithm that ensures the trees stay
+          balanced.  We'll do that in [Redblack].
+
+     2. Our keys are natural numbers, and Coq's [nat] type takes linear
+        time per comparison.  That is, computing (j <? k) takes time
+        proportional to the value of [k-j].
+
+        - SOLUTION: represent keys by a data type that has a more
+          efficient comparison operator.  We used [nat] in this chapter
+          because it's something easy to work with.
+
+     3. There's no notion of running time in Coq.  That is, we can't
+        say what it means that a Coq function "takes N steps to
+        evaluate."  Therefore, we can't prove that binary search trees
+        are efficient.
+
+        - SOLUTION 1: Don't prove (in Coq) that they're efficient;
+          just prove that they are correct.  Prove things about their
+          efficiency the old-fashioned way, on pencil and paper.
+
+        - SOLUTION 2: Prove in Coq some facts about the height of the
+          trees, which have direct bearing on their efficiency.  We'll
+          explore that in [Redblack].
+
+        - SOLUTION 3: Apply bleeding-edge frameworks for reasoning
+          about run-time of programs represented in Coq.
+
+      4. Our functions in Coq are models of implementations in "real"
+         programming languages.  What if the real implementations
+         differ from the Coq models?
+
+         - SOLUTION: Use Coq's [extraction] feature to derive the real
+	   implementation (in Ocaml or Haskell) automatically from the
+	   Coq function.  Or, use Coq's [Compute] or [Eval
+	   native_compute] feature to compile and run the programs
+	   efficiently inside Coq.  We'll explore [extraction] in a
+	   [Extract]. *)
+
+(* 2021-08-11 15:15 *)
