src/theories/Eval.v
@@ -7,7 +7,7 @@ Open Scope bs.
 Require Import Coq.Lists.List.
 Import ListNotations.
 
-Definition coerce {A} (x: (option A)) := 
+Polymorphic Definition coerce {A} (x: (option A)) := 
   match x with 
   | Some v => tmReturn v
   | None => tmFail "coerce"
@@ -18,8 +18,6 @@ Definition is_prop_t (t: term) :=
   | tSort u => Universe.is_prop u
   | _ => false
   end.
-
-Print Universe.is_type_sort.
 
 Definition is_type_t (t: term) := 
   match t with 
@@ -34,6 +32,12 @@ Definition is_set_t (t: term) :=
   end.
 
 Definition is_fo_kind (t: term) := (is_type_t t || is_set_t t)%bool.
+
+Polymorphic Fixpoint is_prop_prod (t: term) := 
+  match t with 
+  | tProd _ _ b => is_prop_prod b
+  | _ => is_prop_t t
+  end.
 
 Definition check_ind_params (t: mutual_inductive_body) := 
   List.fold_left 
@@ -76,7 +80,7 @@ Fixpoint make_param_prefix (ctx: fo_context) (n: nat) : fo_context :=
   | S n' => (tRel n, true) :: make_param_prefix ctx n'
   end.
 
-Fixpoint validate_fo_type (ctx: fo_context) (t: term) : option bool := 
+Polymorphic Fixpoint validate_fo_type (ctx: fo_context) (t: term) : option bool := 
   match t with 
   | tApp f xs => 
     let inner := (let fix rec acc := 
@@ -119,6 +123,81 @@ Fixpoint opt_seq {A} (xs : list (option A)) : option (list A) :=
   | None :: _ => None
   end.
 
+Require MirrorSolve.Reflection.FM.
+
+Polymorphic Fixpoint validate_fo_term (ctx_ty: fo_context) (ctx_term: fo_context) (t: term) : option bool :=
+  match t with 
+  | tApp _ es => 
+    let worker t := 
+      match validate_fo_term ctx_ty ctx_term t with 
+      | Some b => Some b
+      | None => validate_fo_type ctx_ty t
+      end in 
+    match opt_seq (map worker es) with 
+    | Some bs' => Some (all_bool bs')
+    | None => None
+    end
+  | _ => find _ _ eq_term t ctx_term
+  end.
+
+Polymorphic Fixpoint validate_fo_prop (ctx_ty: fo_context) (ctx_term: fo_context) (t: term) : option bool := 
+  if (eq_term t FM.c_True || eq_term t FM.c_False)%bool then Some true else
+  match t with
+  | tApp f es => 
+    if eq_term f FM.c_eq then 
+      match es with 
+      | t_ty :: tl :: tr :: _ => validate_fo_type ctx_ty t_ty
+      | _ => None
+      end
+    else if (eq_term f FM.c_or || eq_term f FM.c_and)%bool then 
+      match es with 
+      | tl :: tr :: _ => 
+        match validate_fo_prop ctx_ty ctx_term tl, validate_fo_prop ctx_ty ctx_term tl with 
+        | Some l, Some r => Some (l && r)%bool
+        | _, _ => None
+        end
+      | _ => None
+      end
+    else if eq_term f FM.c_not then 
+      match es with 
+      | x :: _ => validate_fo_prop ctx_ty ctx_term x
+      | _ => None
+      end
+    else
+      let worker t := 
+        match validate_fo_term ctx_ty ctx_term t with 
+        | Some b => Some b
+        | None => validate_fo_type ctx_ty t
+        end in 
+      match opt_seq (map worker es) with 
+      | Some bs' => Some (all_bool bs')
+      | None => None
+      end
+  | tProd ba_name ty bod =>
+    match ba_name.(binder_name) with 
+    | nAnon => 
+      match validate_fo_prop ctx_ty ctx_term ty, validate_fo_prop ctx_ty (map Utils.inc_subst_var ctx_term) bod with 
+      | Some el, Some er => Some (el && er)%bool
+      | _, _ => None
+      end
+    | nNamed _ => 
+      match validate_fo_type ctx_ty ty with 
+      | Some b_ty => 
+        let ctx_term' := (tRel 0, b_ty) :: (map Utils.inc_subst_var ctx_term) in 
+        validate_fo_prop ctx_ty ctx_term' bod
+      | None => None
+      end
+    end
+  | _ => None
+  end.
+
+Polymorphic Fixpoint norm_lambda (t: term) : term := 
+  match t with 
+  | tLambda name ty bod => 
+    tProd name ty (norm_lambda bod)
+  | _ => t
+  end.
+
 Definition validate_fo_ind (ctx: fo_context) (ind: one_inductive_body) (parent: mutual_inductive_body) := 
   (* assume the original ind type and also the indices are valid FO-types *)
   let param_len := length parent.(ind_params) in 
@@ -139,28 +218,151 @@ Definition validate_fo_ind (ctx: fo_context) (ind: one_inductive_body) (parent: 
   | _ => None
   end.
 
-Definition run_add (ctx: fo_context) (t: term) : TemplateMonad (option fo_context) :=
+Polymorphic Definition run_once_type (ctx: fo_context) (t: term) : TemplateMonad (option bool) :=
   match t with 
   | tInd ind _ => 
     inds <- tmQuoteInductive ind.(inductive_mind) ;;
     ind' <- coerce (nth_error inds.(ind_bodies) ind.(inductive_ind)) ;;
+    if is_prop_prod (ind'.(ind_type)) then tmReturn None else
     let ctx_inner := make_param_prefix ctx (length inds.(ind_params)) in 
-    match validate_fo_ind ctx_inner ind' inds with 
-    | Some b => tmReturn (Some ((t, b) :: ctx))
-    | None => tmReturn None
-    end
-  | _ => tmFail "run_add"
+    tmReturn (validate_fo_ind ctx_inner ind' inds)
+  | _ => 
+    tmReturn (validate_fo_type ctx t)
   end.
 
-(* Print constant_body. *)
+Definition builtin_names := [
+      (MPfile ["BinNums"; "Numbers"; "Coq"], "Z")
+    ; (MPfile ["Datatypes"; "Init"; "Coq"], "bool")
+  ].
 
-(* End-to-end algorithm:
+Polymorphic Definition handle_one_decl (ctx: fo_context) (g: kername * global_decl) : TemplateMonad (option fo_context) := 
+  match g.2 with 
+  | ConstantDecl _ => 
+    (* tmPrint "skipping const decl for" ;; 
+    x <- tmEval all g.1 ;; 
+    tmPrint x ;; *)
+    tmReturn (Some ctx)
+  | InductiveDecl mi_bod => 
+    tmReturn (
+    if inb _ eq_kername g.1 builtin_names then Some ((tInd (mkInd g.1 0) [], true) :: ctx)
+    else
+    match mi_bod.(ind_bodies) with 
+    | [ind'] => 
+      if is_prop_prod ind'.(ind_type) then Some ctx else
+      let ctx_inner := make_param_prefix ctx (length mi_bod.(ind_params)) in 
+        match validate_fo_ind ctx_inner ind' mi_bod with 
+        | Some b => Some ((tInd (mkInd g.1 0) [], b) :: ctx)
+        | None => None
+        end
+    | _ => Some ctx
+    end)
+  end.
 
-  1) quote recursively;
-  2) add each declaration, in order, to a first-order typing context
-    2a) special-case nat, bool, Z, N, and pos
-    2b) handle inductives using the definition above
-    2c) skip definitions
-    2d) figure out section variables...not sure how they present
-  3) lookup and return the original term's value in the resulting context
-*)
+Polymorphic Definition handle_decls_worker (acc: option fo_context ) (d: kername * global_decl) : TemplateMonad (option fo_context) := 
+  match acc with 
+  | Some acc' => handle_one_decl acc' d 
+  | _ => tmReturn None
+  end.
+
+Polymorphic Definition handle_all_decls (ctx: fo_context) (gs: list (kername * global_decl)) : TemplateMonad (option fo_context) := 
+  foldlM handle_decls_worker (Some ctx) gs.
+
+Polymorphic Definition get_type {A} (_: A) : TemplateMonad term := 
+  tmQuote A.
+
+Polymorphic Definition get_type_term (x: term) : TemplateMonad term := 
+  x <- tmUnquote x ;;
+  x <- tmEval all x.(my_projT1) ;;
+  tmQuote x.
+
+Polymorphic Fixpoint extract_vars (t: term) : list term := 
+  match t with 
+  | tVar _ => [t]
+  | tProd _ ty bod => extract_vars ty ++ extract_vars bod
+  | tLambda _ ty bod => extract_vars ty ++ extract_vars bod
+  | tLetIn _ ty v bod => extract_vars ty ++ extract_vars v ++ extract_vars bod
+  | tApp f args => 
+    extract_vars f ++ List.concat (List.map extract_vars args)
+  | tProj _ x => extract_vars x
+  | _ => []
+  end.
+
+Polymorphic Definition preprocess_vars (t: term) : TemplateMonad fo_context := 
+  mapM (fun x => ty <- get_type_term x ;; tmReturn (x, is_fo_kind ty)) (uniq _ eq_term (extract_vars t)).
+
+
+Polymorphic Definition is_fo_type (p: program) : TemplateMonad (option bool) :=
+  (* tmPrint "decls:" ;; 
+  x <- tmEval all p.1.(declarations) ;; 
+  tmPrint x ;; *)
+  ctx <- preprocess_vars p.2 ;;
+  (* tmPrint "init ctx:" ;; 
+  x <- tmEval all ctx ;; 
+  tmPrint x ;; *)
+  r <- handle_all_decls ctx (List.rev (p.1.(declarations)));;
+  match r with 
+  | Some ctx' => 
+    (* tmPrint "ctx:" ;; 
+    tmPrint ctx' ;;
+    tmPrint "term:" ;; 
+    x <- tmEval all p.2 ;;
+    tmPrint x ;; *)
+    run_once_type ctx' p.2
+  | None => tmReturn None
+  end.
+
+
+Polymorphic Definition quoteConstRec {A} (a: A) : TemplateMonad program := 
+  x <- tmQuote a ;; 
+  match x with 
+  | tConst name _ => 
+    y <- tmQuoteConstant name false ;; 
+    match y.(cst_body) with 
+    | Some t => 
+      inter <- tmUnquote t ;; 
+      inter <- tmEval all (my_projT2 inter) ;;
+      tmQuoteRec inter
+    | _ => 
+      tmPrint x ;;
+      tmFail "opaque/undefined constant in quoteConstRec"
+    end
+  | _ => 
+    tmPrint x ;; 
+    tmFail "quoteConstRec passed a non-constant input"
+  end.
+
+Polymorphic Definition is_fo_const {A} (a: A) : TemplateMonad (option bool) := 
+  p <- quoteConstRec a ;;
+  let t := norm_lambda p.2 in 
+  ctx <- preprocess_vars t ;;
+  (* tmPrint "init ctx:" ;; 
+  x <- tmEval all ctx ;; 
+  tmPrint x ;; *)
+  r <- handle_all_decls ctx (List.rev (p.1.(declarations))) ;;
+  match r with 
+  | Some ctx' => tmReturn (validate_fo_prop ctx' [] t)
+  | _ => tmReturn None
+  end.
+
+(* Section Foo.
+Variable (X: Type).
+Definition foo := forall (x: X), (fun y => y = x) = (fun z => z = x).
+
+MetaCoq Run (
+  MetaCoq.Template.TemplateMonad.Core.tmBind (is_fo_const foo)  (fun x => 
+  MetaCoq.Template.TemplateMonad.Core.tmBind (MetaCoq.Template.TemplateMonad.Core.tmEval MetaCoq.Template.TemplateMonad.Common.all x) (fun x => 
+  MetaCoq.Template.TemplateMonad.Core.tmPrint x
+))). *)
+
+(* Section Foo.
+Variable (A: Type).
+Variable (B: Type).
+Variable f: A -> B.
+
+MetaCoq Run (
+  x <- tmQuote (A, B, f) ;;
+  x <- preprocess_vars x ;;
+  x <- tmEval all x ;; 
+  tmPrint x
+). *)
+
